Denotation/theories/TypeDenote.v
@@ -1,28 +1,28 @@
-(** * Denotation.ContextTypeDenotationDefinition *)
+(** * Denotation.TypeDenote *)
 
 From Denotation Require Import Notation.
 
-Section ContextTypeDenotation.
+Section TypeDenote.
 
-Definition denot_guard_formula
+Definition ty_guard_formula
     (Σ : lty_env) (τ : context_ty) (e : tm) : FormulaT :=
   FAnd (context_ty_wf_formula Σ τ)
     (FAnd (basic_world_formula Σ)
       (FAnd (expr_basic_typing_formula Σ e (erase_ty τ))
             (expr_total_formula e))).
 
-Definition denot_static_guard_formula
+Definition ty_static_guard_formula
     (Σ : lty_env) (τ : context_ty) (e : tm) : FormulaT :=
   FAnd (context_ty_wf_formula Σ τ)
     (FAnd (basic_world_formula Σ)
       (expr_basic_typing_formula Σ e (erase_ty τ))).
 
-Fixpoint denot_ty_lvar_gas
+Fixpoint ty_denote_gas
     (gas : nat) (Σ : lty_env) (τ : context_ty) (e : tm)
     {struct gas} : FormulaT :=
   let Σg := denot_relevant_env Σ τ e in
   FAnd
-    (denot_guard_formula Σg τ e)
+    (ty_guard_formula Σg τ e)
     (match gas with
     | 0 => FTrue
     | S gas' =>
@@ -43,33 +43,33 @@ Fixpoint denot_ty_lvar_gas
                   (FUnder (type_qualifier_formula φ)))))
       | CTInter τ1 τ2 =>
           FAnd
-            (denot_ty_lvar_gas gas' Σ τ1 e)
-            (denot_ty_lvar_gas gas' Σ τ2 e)
+            (ty_denote_gas gas' Σ τ1 e)
+            (ty_denote_gas gas' Σ τ2 e)
       | CTUnion τ1 τ2 =>
           FOr
-            (denot_ty_lvar_gas gas' Σ τ1 e)
-            (denot_ty_lvar_gas gas' Σ τ2 e)
+            (ty_denote_gas gas' Σ τ1 e)
+            (ty_denote_gas gas' Σ τ2 e)
       | CTSum τ1 τ2 =>
           FPlus
-            (denot_ty_lvar_gas gas' Σ τ1 e)
-            (denot_ty_lvar_gas gas' Σ τ2 e)
+            (ty_denote_gas gas' Σ τ1 e)
+            (ty_denote_gas gas' Σ τ2 e)
       | CTArrow τx τr =>
           let Σx := typed_lty_env_bind Σg (erase_ty τx) in
           FForall
             (FImpl (basic_world_formula (<[LVBound 0 := (erase_ty τx)]> ∅))
               (FImpl
-                (denot_ty_lvar_gas gas' Σx
+                (ty_denote_gas gas' Σx
                   (cty_shift 0 τx) (tret (vbvar 0)))
-                (denot_ty_lvar_gas gas' Σx τr
+                (ty_denote_gas gas' Σx τr
                   (tapp_tm (tm_shift 0 e) (vbvar 0)))))
       | CTWand τx τr =>
           let Σx := typed_lty_env_bind Σg (erase_ty τx) in
           FForall
             (FImpl (basic_world_formula (<[LVBound 0 := (erase_ty τx)]> ∅))
               (FWand
-                (denot_ty_lvar_gas gas' Σx
+                (ty_denote_gas gas' Σx
                   (cty_shift 0 τx) (tret (vbvar 0)))
-                (denot_ty_lvar_gas gas' Σx τr
+                (ty_denote_gas gas' Σx τr
                   (tapp_tm (tm_shift 0 e) (vbvar 0)))))
     end
     end).
@@ -89,15 +89,15 @@ Lemma formula_open_env_denot_guard η Σ τ e :
   open_env_fresh_for_lvars η (dom Σ ∪ denot_relevant_lvars τ e) ->
   open_env_values_inj η ->
   formula_open_env η
-    (denot_guard_formula (denot_relevant_env Σ τ e) τ e) =
-  denot_guard_formula
+    (ty_guard_formula (denot_relevant_env Σ τ e) τ e) =
+  ty_guard_formula
     (denot_relevant_env (lty_env_open_lvars η Σ)
       (open_cty_env η τ) (open_tm_env η e))
     (open_cty_env η τ)
     (open_tm_env η e).
 Proof.
   intros Hfresh Hinj.
-  unfold denot_guard_formula.
+  unfold ty_guard_formula.
   rewrite !formula_open_env_and.
   rewrite formula_open_env_context_ty_wf_formula.
   2:{
@@ -138,17 +138,17 @@ Proof.
   reflexivity.
 Qed.
 
-Lemma formula_open_env_denot_ty_lvar_gas_zero η Σ τ e :
+Lemma formula_open_env_ty_denote_gas_zero η Σ τ e :
   open_env_fresh_for_lvars η (dom Σ ∪ denot_relevant_lvars τ e) ->
   open_env_values_inj η ->
-  formula_open_env η (denot_ty_lvar_gas 0 Σ τ e) =
-  denot_ty_lvar_gas 0
+  formula_open_env η (ty_denote_gas 0 Σ τ e) =
+  ty_denote_gas 0
     (lty_env_open_lvars η Σ)
     (open_cty_env η τ)
     (open_tm_env η e).
 Proof.
   intros Hfresh Hinj.
-  cbn [denot_ty_lvar_gas].
+  cbn [ty_denote_gas].
   rewrite formula_open_env_and.
   rewrite formula_open_env_denot_guard by (exact Hfresh || exact Hinj).
   rewrite formula_open_env_true.
@@ -174,12 +174,12 @@ Ltac denot_open_env_qual_case η Hfresh Hinj φ e :=
   | assert (Hfreshe : open_env_fresh_for_lvars η (tm_lvars e));
     [ eapply open_env_fresh_for_lvars_mono; [|exact Hfresh];
       unfold denot_relevant_lvars; set_solver
-    | cbn [denot_ty_lvar_gas];
+    | cbn [ty_denote_gas];
       rewrite formula_open_env_and;
       rewrite formula_open_env_denot_guard by (exact Hfresh || exact Hinj);
       first [rewrite open_cty_env_over by exact Hinj
             |rewrite open_cty_env_under by exact Hinj];
-      cbn [denot_ty_lvar_gas];
+      cbn [ty_denote_gas];
       rewrite formula_open_env_forall by exact Hinj;
       rewrite !formula_open_env_impl;
       rewrite formula_open_env_basic_world_formula;
@@ -200,13 +200,13 @@ Ltac denot_open_env_qual_case η Hfresh Hinj φ e :=
       |apply open_env_values_inj_lift; exact Hinj] ] ].
 
 Ltac denot_open_env_binary_case IH Hfresh Hinj :=
-  cbn [denot_ty_lvar_gas];
+  cbn [ty_denote_gas];
   rewrite formula_open_env_and;
   rewrite formula_open_env_denot_guard by (exact Hfresh || exact Hinj);
   first [rewrite open_cty_env_inter
         |rewrite open_cty_env_union
         |rewrite open_cty_env_sum];
-  cbn [denot_ty_lvar_gas];
+  cbn [ty_denote_gas];
   first [rewrite formula_open_env_and
         |rewrite formula_open_env_or
         |rewrite formula_open_env_plus];
@@ -215,11 +215,11 @@ Ltac denot_open_env_binary_case IH Hfresh Hinj :=
   rewrite (IH _ _ _ _);
   [reflexivity|denot_open_env_child_fresh Hfresh|exact Hinj].
 
-Lemma formula_open_env_denot_ty_lvar_gas η gas Σ τ e :
+Lemma formula_open_env_ty_denote_gas η gas Σ τ e :
   open_env_fresh_for_lvars η (dom Σ ∪ denot_relevant_lvars τ e) ->
   open_env_values_inj η ->
-  formula_open_env η (denot_ty_lvar_gas gas Σ τ e) =
-  denot_ty_lvar_gas gas
+  formula_open_env η (ty_denote_gas gas Σ τ e) =
+  ty_denote_gas gas
     (lty_env_open_lvars η Σ)
     (open_cty_env η τ)
     (open_tm_env η e).
@@ -229,7 +229,7 @@ Proof.
      [formula_open_env_forall] with [(kmap S η)]. *)
   revert Σ τ e η.
   induction gas as [|gas IH]; intros Σ τ e η Hfresh Hinj.
-  - apply formula_open_env_denot_ty_lvar_gas_zero; assumption.
+  - apply formula_open_env_ty_denote_gas_zero; assumption.
   - destruct τ as [b φ|b φ|τ1 τ2|τ1 τ2|τ1 τ2|τx τr|τx τr].
     + denot_open_env_qual_case η Hfresh Hinj φ e.
     + denot_open_env_qual_case η Hfresh Hinj φ e.
@@ -266,11 +266,11 @@ Proof.
         eapply open_env_fresh_for_lvars_mono; [|exact Hfresh].
         apply lvars_at_depth_arrow_body_lift_support_subset.
       }
-      cbn [denot_ty_lvar_gas].
+      cbn [ty_denote_gas].
       rewrite formula_open_env_and.
       rewrite formula_open_env_denot_guard by (exact Hfresh || exact Hinj).
       rewrite open_cty_env_arrow by exact Hinj.
-      cbn [denot_ty_lvar_gas].
+      cbn [ty_denote_gas].
       rewrite formula_open_env_forall by exact Hinj.
       rewrite !formula_open_env_impl.
       rewrite formula_open_env_basic_world_formula.
@@ -329,11 +329,11 @@ Proof.
         eapply open_env_fresh_for_lvars_mono; [|exact Hfresh].
         apply lvars_at_depth_wand_body_lift_support_subset.
       }
-      cbn [denot_ty_lvar_gas].
+      cbn [ty_denote_gas].
       rewrite formula_open_env_and.
       rewrite formula_open_env_denot_guard by (exact Hfresh || exact Hinj).
       rewrite open_cty_env_wand by exact Hinj.
-      cbn [denot_ty_lvar_gas].
+      cbn [ty_denote_gas].
       rewrite formula_open_env_forall by exact Hinj.
       rewrite formula_open_env_impl.
       rewrite formula_open_env_wand.
@@ -365,19 +365,19 @@ Proof.
       reflexivity.
 Qed.
 
-Lemma denot_ty_lvar_gas_env_agree_on gas Σ1 Σ2 τ e X :
+Lemma ty_denote_gas_env_agree_on gas Σ1 Σ2 τ e X :
   denot_relevant_lvars τ e ⊆ X ->
   lty_env_restrict_lvars Σ1 X = lty_env_restrict_lvars Σ2 X ->
-  denot_ty_lvar_gas gas Σ1 τ e =
-  denot_ty_lvar_gas gas Σ2 τ e.
+  ty_denote_gas gas Σ1 τ e =
+  ty_denote_gas gas Σ2 τ e.
 Proof.
   induction gas as [|gas IH] in Σ1, Σ2, τ, e, X |- *; intros Hsub Heq.
-  - cbn [denot_ty_lvar_gas].
+  - cbn [ty_denote_gas].
     unfold denot_relevant_env, lty_env_restrict_lvars.
     erewrite storeA_restrict_eq_mono by (exact Hsub || exact Heq).
     reflexivity.
   - destruct τ as [b φ|b φ|τ1 τ2|τ1 τ2|τ1 τ2|τ1 τ2|τ1 τ2];
-      cbn [denot_ty_lvar_gas].
+      cbn [ty_denote_gas].
     + unfold denot_relevant_env, lty_env_restrict_lvars.
       erewrite storeA_restrict_eq_mono by (exact Hsub || exact Heq).
       reflexivity.
@@ -437,23 +437,23 @@ Proof.
       reflexivity.
 Qed.
 
-Lemma res_models_denot_ty_lvar_gas_env_agree_on
+Lemma res_models_ty_denote_gas_env_agree_on
     gas Σ1 Σ2 τ e X (m : WfWorldT) :
   denot_relevant_lvars τ e ⊆ X ->
   lty_env_restrict_lvars Σ1 X = lty_env_restrict_lvars Σ2 X ->
-  m ⊨ denot_ty_lvar_gas gas Σ1 τ e ->
-  m ⊨ denot_ty_lvar_gas gas Σ2 τ e.
+  m ⊨ ty_denote_gas gas Σ1 τ e ->
+  m ⊨ ty_denote_gas gas Σ2 τ e.
 Proof.
   intros Hsub Heq Hmodels.
-  rewrite <- (denot_ty_lvar_gas_env_agree_on gas Σ1 Σ2 τ e X Hsub Heq).
+  rewrite <- (ty_denote_gas_env_agree_on gas Σ1 Σ2 τ e X Hsub Heq).
   exact Hmodels.
 Qed.
 
-End ContextTypeDenotation.
+End TypeDenote.
 
 (** ** Free-variable support for denotation formulas *)
 
-Section ContextTypeDenotationSupport.
+Section TypeDenoteSupport.
 
 Ltac rewrite_tm_support :=
   repeat match goal with
@@ -464,7 +464,7 @@ Ltac rewrite_tm_support :=
   end.
 
 Ltac unfold_formula_lvars_atoms :=
-  unfold denot_guard_formula;
+  unfold ty_guard_formula;
   cbn [formula_lvars_at context_ty_wf_formula basic_world_formula
     expr_basic_typing_formula expr_total_formula expr_result_formula
     type_qualifier_formula];
@@ -487,12 +487,12 @@ Ltac normalize_denot_formula_lvars :=
   rewrite ?lvars_at_depth_empty;
   cbn [context_ty_lvars_at tm_lvars_at value_lvars_at].
 
-Lemma formula_lvars_at_denot_ty_lvar_gas_subset_relevant gas d Σ τ e :
-  formula_lvars_at d (denot_ty_lvar_gas gas Σ τ e) ⊆
+Lemma formula_lvars_at_ty_denote_gas_subset_relevant gas d Σ τ e :
+  formula_lvars_at d (ty_denote_gas gas Σ τ e) ⊆
   tm_lvars_at d e ∪ context_ty_lvars_at d τ.
 Proof.
   induction gas as [|gas IH] in d, Σ, τ, e |- *.
-  - cbn [denot_ty_lvar_gas formula_lvars_at].
+  - cbn [ty_denote_gas formula_lvars_at].
     normalize_denot_formula_lvars.
     pose proof (lvars_at_depth_denot_relevant_env_subset_relevant d Σ τ e).
     intros v Hv.
@@ -506,7 +506,7 @@ Proof.
     + tauto.
     + tauto.
   - destruct τ as [b φ|b φ|τ1 τ2|τ1 τ2|τ1 τ2|τ1 τ2|τ1 τ2];
-      cbn [denot_ty_lvar_gas formula_lvars_at].
+      cbn [ty_denote_gas formula_lvars_at].
     + normalize_denot_formula_lvars.
       pose proof (lvars_at_depth_denot_relevant_env_subset_relevant d Σ (CTOver b φ) e).
       pose proof (lvars_at_depth_mono (S d)
@@ -595,8 +595,8 @@ Proof.
       set_solver.
 Qed.
 
-Lemma formula_fv_denot_ty_lvar_gas_subset_relevant_pre_open gas Σ τ e :
-  formula_fv (denot_ty_lvar_gas gas Σ τ e) ⊆
+Lemma formula_fv_ty_denote_gas_subset_relevant_pre_open gas Σ τ e :
+  formula_fv (ty_denote_gas gas Σ τ e) ⊆
   fv_tm e ∪ fv_cty τ.
 Proof.
   rewrite <- (formula_lvars_at_fv 0).
@@ -604,14 +604,14 @@ Proof.
   - apply lvars_fv_mono.
     unfold denot_relevant_lvars.
     transitivity (tm_lvars_at 0 e ∪ context_ty_lvars_at 0 τ).
-    + apply formula_lvars_at_denot_ty_lvar_gas_subset_relevant.
+    + apply formula_lvars_at_ty_denote_gas_subset_relevant.
     + change (tm_lvars_at 0 e) with (tm_lvars e).
       change (context_ty_lvars_at 0 τ) with (context_ty_lvars τ).
       set_solver.
   - rewrite denot_relevant_lvars_fv. set_solver.
 Qed.
 
-Lemma formula_fv_denot_ty_lvar_gas_scope_from_guard_pre_open
+Lemma formula_fv_ty_denote_gas_scope_from_guard_pre_open
     gas Σ τsmall τbig e (m : WfWorldT) :
   context_ty_lvars τsmall ⊆ context_ty_lvars τbig ->
   m ⊨ FAnd
@@ -621,13 +621,13 @@ Lemma formula_fv_denot_ty_lvar_gas_scope_from_guard_pre_open
         (expr_basic_typing_formula (denot_relevant_env Σ τbig e) e
           (erase_ty τbig))
         (expr_total_formula e))) ->
-  formula_fv (denot_ty_lvar_gas gas Σ τsmall e) ⊆ world_dom (m : WorldT).
+  formula_fv (ty_denote_gas gas Σ τsmall e) ⊆ world_dom (m : WorldT).
 Proof.
   intros Hτ Hguard.
   repeat rewrite res_models_and_iff in Hguard.
   destruct Hguard as [Hwf [Hworld [_ Htotal_e]]].
   transitivity (fv_tm e ∪ fv_cty τsmall).
-  - apply formula_fv_denot_ty_lvar_gas_subset_relevant_pre_open.
+  - apply formula_fv_ty_denote_gas_subset_relevant_pre_open.
   - pose proof (res_models_fuel_scoped _ _ _ Htotal_e) as Hscope_e.
     unfold formula_scoped_in_world in Hscope_e.
     rewrite formula_fv_expr_total_formula, tm_lvars_fv in Hscope_e.
@@ -644,4 +644,4 @@ Proof.
     set_solver.
 Qed.
 
-End ContextTypeDenotationSupport.
+End TypeDenoteSupport.
