Denotation/theories/TypeDenoteOpen.v
@@ -1,22 +1,22 @@
-(** * Denotation.ContextTypeDenotationOpen *)
+(** * Denotation.TypeDenoteOpen *)
 
 From Denotation Require Import Notation.
-From Denotation Require Import ContextTypeDenotationTactics.
-From Denotation Require Export ContextTypeDenotationDefinition.
+From Denotation Require Import TypeDenoteTactics.
+From Denotation Require Export TypeDenote.
 
-Section ContextTypeDenotation.
+Section TypeDenote.
 
-Definition denot_ty
+Definition ty_denote
     (Δ : gmap atom ty) (τ : context_ty) (e : tm) : FormulaT :=
-  denot_ty_lvar_gas (cty_depth τ) (atom_env_to_lty_env Δ) τ e.
+  ty_denote_gas (cty_depth τ) (atom_env_to_lty_env Δ) τ e.
 
-Lemma formula_open_denot_ty_lvar_gas_singleton
+Lemma formula_open_ty_denote_gas_singleton
     k y gas Σ τ e :
   y ∉ lvars_fv (dom Σ) ->
   y ∉ fv_tm e ->
   y ∉ fv_cty τ ->
-  formula_open k y (denot_ty_lvar_gas gas Σ τ e) =
-  denot_ty_lvar_gas gas
+  formula_open k y (ty_denote_gas gas Σ τ e) =
+  ty_denote_gas gas
     (lty_env_open_one k y Σ)
     (cty_open k y τ)
     (open_tm k (vfvar y) e).
@@ -31,7 +31,7 @@ Proof.
     open_env_fresh_for_lvars (<[k := y]> ∅)
       (dom Σ ∪ denot_relevant_lvars τ e)).
   { denot_open_set. }
-  pose proof (formula_open_env_denot_ty_lvar_gas
+  pose proof (formula_open_env_ty_denote_gas
     (<[k := y]> ∅) gas Σ τ e Hfresh
     (open_env_values_inj_singleton k y)) as Heq.
   rewrite formula_open_env_singleton in Heq.
@@ -41,4 +41,4 @@ Proof.
   exact Heq.
 Qed.
 
-End ContextTypeDenotation.
+End TypeDenote.
