Denotation/theories/TypeEquiv.v
@@ -1,84 +1,84 @@
-(** * Denotation.ContextTypeDenotationSaturateMain
+(** * Denotation.TypeEquiv
 
     Main term-result-equivalence transport theorem. *)
 
-From Denotation Require Import Notation ContextTypeDenotationOpen.
+From Denotation Require Import Notation TypeDenoteOpen.
 From Denotation Require Import
-  ContextTypeDenotationSaturateCore
-  ContextTypeDenotationSaturateBody
-  ContextTypeDenotationSaturateArrow
-  ContextTypeDenotationSaturateWand.
+  TypeEquivCore
+  TypeEquivBody
+  TypeEquivArrow
+  TypeEquivWand.
 
-Section ContextTypeDenotation.
+Section TypeDenote.
 
-Lemma denot_ty_lvar_gas_tm_result_equiv
+Lemma ty_denote_gas_tm_equiv
     gas Σ τ e1 e2 (m : WfWorldT) :
-  typed_total_tm_result_equiv_on Σ τ m e1 e2 ->
-  m ⊨ denot_ty_lvar_gas gas Σ τ e1 ->
-  m ⊨ denot_ty_lvar_gas gas Σ τ e2.
+  typed_total_equiv_on Σ τ m e1 e2 ->
+  m ⊨ ty_denote_gas gas Σ τ e1 ->
+  m ⊨ ty_denote_gas gas Σ τ e2.
 Proof.
   revert Σ τ e1 e2 m.
   induction gas as [|gas IH]; intros Σ τ e1 e2 m Hequiv Hm.
-  - exact (typed_total_tm_result_equiv_on_target_zero _ _ _ _ _ Hequiv).
-  - pose proof (typed_total_tm_result_equiv_on_target_zero
+  - exact (typed_total_equiv_target_zero _ _ _ _ _ Hequiv).
+  - pose proof (typed_total_equiv_target_zero
       Σ τ m e1 e2 Hequiv) as Hzero_tgt.
-    pose proof (denot_ty_lvar_gas_guard_of_zero
+    pose proof (ty_denote_gas_guard_of_zero
       Σ τ e2 m Hzero_tgt) as Hguard_tgt.
     repeat rewrite res_models_and_iff in Hguard_tgt.
 	    destruct τ as [b φ|b φ|τ1 τ2|τ1 τ2|τ1 τ2|τx τr|τx τr];
-	      cbn [denot_ty_lvar_gas denot_guard_formula] in Hm |- *;
-	      unfold denot_guard_formula in Hm |- *;
+	      cbn [ty_denote_gas ty_guard_formula] in Hm |- *;
+	      unfold ty_guard_formula in Hm |- *;
 	      repeat rewrite res_models_and_iff in Hm |- *;
 	      destruct Hm as [_ Hbody]; split.
 		    all: try exact Hguard_tgt.
-	    + eapply denot_ty_lvar_gas_tm_result_equiv_over_body; eauto.
-	    + eapply denot_ty_lvar_gas_tm_result_equiv_under_body; eauto.
-	    + eapply denot_ty_lvar_gas_tm_result_equiv_inter_body; eauto.
-	    + eapply denot_ty_lvar_gas_tm_result_equiv_union_body; eauto.
-	    + eapply denot_ty_lvar_gas_tm_result_equiv_sum_body; eauto.
-	    + eapply denot_ty_lvar_gas_tm_result_equiv_arrow_body; eauto.
-	    + eapply denot_ty_lvar_gas_tm_result_equiv_wand_body; eauto.
+	    + eapply ty_denote_gas_tm_equiv_over_body; eauto.
+	    + eapply ty_denote_gas_tm_equiv_under_body; eauto.
+	    + eapply ty_denote_gas_tm_equiv_inter_body; eauto.
+	    + eapply ty_denote_gas_tm_equiv_union_body; eauto.
+	    + eapply ty_denote_gas_tm_equiv_sum_body; eauto.
+	    + eapply ty_denote_gas_tm_equiv_arrow_body; eauto.
+	    + eapply ty_denote_gas_tm_equiv_wand_body; eauto.
 	Qed.
 
-Lemma denot_ty_lvar_gas_result_alias_to_var
+Lemma ty_denote_gas_result_alias
     gas (Σ : lty_env) τ e x (m : WfWorldT) :
   lty_env_closed Σ ->
   Σ !! LVFree x = Some (erase_ty τ) ->
   m ⊨ expr_result_formula e (LVFree x) ->
-  m ⊨ denot_ty_lvar_gas gas Σ τ e ->
-  m ⊨ denot_ty_lvar_gas gas Σ τ (tret (vfvar x)).
+  m ⊨ ty_denote_gas gas Σ τ e ->
+  m ⊨ ty_denote_gas gas Σ τ (tret (vfvar x)).
 Proof.
   intros HΣclosed HΣx Hres Hm.
-  pose proof (denot_ty_lvar_gas_guard gas Σ τ e m Hm) as Hguard_src.
-  pose proof (denot_ty_lvar_gas_result_alias_guard
+  pose proof (ty_denote_gas_guard gas Σ τ e m Hm) as Hguard_src.
+  pose proof (ty_denote_gas_result_alias_guard
     Σ τ e x m HΣclosed HΣx Hres Hguard_src) as Hguard_tgt.
-  pose proof (denot_ty_lvar_gas_zero_of_guard Σ τ e m Hguard_src)
+  pose proof (ty_denote_gas_zero_of_guard Σ τ e m Hguard_src)
     as Hzero_src.
-  pose proof (denot_ty_lvar_gas_zero_of_guard
+  pose proof (ty_denote_gas_zero_of_guard
     Σ τ (tret (vfvar x)) m Hguard_tgt) as Hzero_tgt.
   pose proof Hguard_tgt as Hguard_tgt_parts.
   repeat rewrite res_models_and_iff in Hguard_tgt_parts.
   destruct Hguard_tgt_parts as [_ [_ [_ Htotal_tgt]]].
-  eapply denot_ty_lvar_gas_tm_result_equiv.
+  eapply ty_denote_gas_tm_equiv.
   - split.
-    + eapply tm_result_equiv_on_result_alias; eauto.
+    + eapply tm_equiv_result_alias; eauto.
     + split; [exact Hzero_src | exact Hzero_tgt].
   - exact Hm.
 Qed.
 
-Lemma denot_ty_lvar_gas_result_extension_to_var
+Lemma ty_denote_gas_result_ext
     gas (Σ : lty_env) τ e x
     (m mx : WfWorldT) (Fx : FiberExtensionT) :
   lty_env_closed Σ ->
   LVFree x ∉ dom Σ ->
   expr_result_extension_witness e x Fx ->
   res_extend_by m Fx mx ->
-  m ⊨ denot_ty_lvar_gas gas Σ τ e ->
-  mx ⊨ denot_ty_lvar_gas gas
+  m ⊨ ty_denote_gas gas Σ τ e ->
+  mx ⊨ ty_denote_gas gas
     (<[LVFree x := erase_ty τ]> Σ) τ (tret (vfvar x)).
 Proof.
   intros HΣclosed HxΣ HFx Hext Hm.
-  pose proof (denot_ty_lvar_gas_guard gas Σ τ e m Hm) as Hguard_full.
+  pose proof (ty_denote_gas_guard gas Σ τ e m Hm) as Hguard_full.
   pose proof Hguard_full as Hguard_parts.
   repeat rewrite res_models_and_iff in Hguard_parts.
   destruct Hguard_parts as [Hwf [Hworld [Hbasic Htotal]]].
@@ -101,7 +101,7 @@ Proof.
       [exact HΣclosed|exact HxΣ|exact HFx|exact Hext|].
     exact Hguard_full.
   }
-  pose proof (denot_ty_lvar_gas_extend_typed_extension
+  pose proof (ty_denote_gas_extend_typed_extension
     gas Σ τ e x (erase_ty τ) m mx Fx
     HxΣ Hxτ Hxe HFx_ltype Hext Hm) as Hmx_source.
   assert (Hfv_e :
@@ -117,19 +117,19 @@ Proof.
     eapply expr_result_formula_of_result_extends
       with (Σ := denot_relevant_env Σ τ e); eauto.
   }
-  eapply denot_ty_lvar_gas_result_alias_to_var; eauto.
+  eapply ty_denote_gas_result_alias; eauto.
   - apply lty_env_closed_insert_free; eauto.
   - apply map_lookup_insert.
 Qed.
 
-Lemma formula_fv_denot_ty_lvar_gas_subset_relevant gas Σ τ e :
-  formula_fv (denot_ty_lvar_gas gas Σ τ e) ⊆
+Lemma formula_fv_ty_denote_gas_subset_relevant gas Σ τ e :
+  formula_fv (ty_denote_gas gas Σ τ e) ⊆
   fv_tm e ∪ fv_cty τ.
 Proof.
   rewrite <- (formula_lvars_at_fv 0).
   transitivity (lvars_fv (tm_lvars_at 0 e ∪ context_ty_lvars_at 0 τ)).
   - apply lvars_fv_mono.
-    apply formula_lvars_at_denot_ty_lvar_gas_subset_relevant.
+    apply formula_lvars_at_ty_denote_gas_subset_relevant.
   - change (tm_lvars_at 0 e) with (tm_lvars e).
     change (context_ty_lvars_at 0 τ) with (context_ty_lvars τ).
     replace (tm_lvars e ∪ context_ty_lvars τ)
@@ -141,11 +141,11 @@ Qed.
 
 Lemma denot_ty_lvar_guard_wfworld_closed_on_term
     (Σ : lty_env) τ e (m : WfWorldT) :
-  m ⊨ denot_guard_formula (denot_relevant_env Σ τ e) τ e ->
+  m ⊨ ty_guard_formula (denot_relevant_env Σ τ e) τ e ->
   wfworld_closed_on (fv_tm e) m.
 Proof.
   intros Hguard.
-  unfold denot_guard_formula in Hguard.
+  unfold ty_guard_formula in Hguard.
   repeat rewrite res_models_and_iff in Hguard.
   destruct Hguard as [_ [Hworld [Hbasic _]]].
   eapply denot_relevant_basic_world_typing_wfworld_closed_on_term; eauto.
@@ -156,13 +156,13 @@ Lemma tlet_intro_denotation
   x ∉ fv_tm e2 ->
   expr_result_extension_witness e1 x Fx ->
   res_extend_by m Fx mx ->
-  mx ⊨ denot_ty_lvar_gas 0 Σ τ (e2 ^^ x) ->
-  mx ⊨ denot_ty_lvar_gas 0 Σ τ (tlete e1 e2) ->
-  mx ⊨ denot_ty_lvar_gas gas Σ τ (e2 ^^ x) ->
-  mx ⊨ denot_ty_lvar_gas gas Σ τ (tlete e1 e2).
+  mx ⊨ ty_denote_gas 0 Σ τ (e2 ^^ x) ->
+  mx ⊨ ty_denote_gas 0 Σ τ (tlete e1 e2) ->
+  mx ⊨ ty_denote_gas gas Σ τ (e2 ^^ x) ->
+  mx ⊨ ty_denote_gas gas Σ τ (tlete e1 e2).
 Proof.
   intros Hx_e2 HFx Hext Hzero_body Hzero_tlet Hbody.
-  pose proof (denot_ty_lvar_gas_guard_of_zero
+  pose proof (ty_denote_gas_guard_of_zero
     Σ τ (tlete e1 e2) mx Hzero_tlet) as Hguard_tlet.
   pose proof Hguard_tlet as Hguard_tlet_parts.
   repeat rewrite res_models_and_iff in Hguard_tlet_parts.
@@ -172,12 +172,12 @@ Proof.
   pose proof (basic_tm_has_ltype_lc _ _ _ HlcΣ Hty_tlet) as Hlc_tlet.
   pose proof (denot_ty_lvar_guard_wfworld_closed_on_term
     Σ τ (tlete e1 e2) mx Hguard_tlet) as Hclosed_tlet.
-  eapply denot_ty_lvar_gas_tm_result_equiv.
+  eapply ty_denote_gas_tm_equiv.
   - split.
-    + eapply tm_result_equiv_on_tlete_body_extension; eauto.
+    + eapply tm_equiv_tlete_body_extension; eauto.
     + split; [exact Hzero_body|exact Hzero_tlet].
   - exact Hbody.
 Qed.
 
 
-End ContextTypeDenotation.
+End TypeDenote.
