Denotation/theories/TypeEquivBody.v
@@ -1,15 +1,15 @@
-(** * Denotation.ContextTypeDenotationSaturateBody
+(** * Denotation.TypeEquivBody
 
     Body cases for term-result-equivalence transport. *)
 
-From Denotation Require Import Notation ContextTypeDenotationOpen.
-From Denotation Require Import ContextTypeDenotationSaturateCore.
+From Denotation Require Import Notation TypeDenoteOpen.
+From Denotation Require Import TypeEquivCore.
 
-Section ContextTypeDenotation.
+Section TypeDenote.
 
-Lemma denot_ty_lvar_gas_tm_result_equiv_over_body
+Lemma ty_denote_gas_tm_equiv_over_body
     (gas : nat) (Σ : lty_env) b φ e1 e2 (m : WfWorldT) :
-  typed_total_tm_result_equiv_on Σ (CTOver b φ) m e1 e2 ->
+  typed_total_equiv_on Σ (CTOver b φ) m e1 e2 ->
   m ⊨
     FForall
       (FImpl (basic_world_formula (<[LVBound 0 := TBase b]> ∅))
@@ -26,21 +26,21 @@ Lemma denot_ty_lvar_gas_tm_result_equiv_over_body
             (FOver (type_qualifier_formula φ))))).
 Proof.
   intros Hequiv Hsrc.
-  pose proof (typed_total_tm_result_equiv_on_term_lc_lvars
+  pose proof (typed_total_equiv_term_lc_lvars
     Σ (CTOver b φ) m e1 e2 Hequiv) as [Hlc_e1 Hlc_e2].
-  pose proof (typed_total_tm_result_equiv_on_target_zero
+  pose proof (typed_total_equiv_target_zero
     Σ (CTOver b φ) m e1 e2 Hequiv) as Hzero_tgt.
-  pose proof (denot_ty_lvar_gas_guard_of_zero
+  pose proof (ty_denote_gas_guard_of_zero
     Σ (CTOver b φ) e2 m Hzero_tgt) as Hguard_tgt.
   assert (Hscope_tgt :
       formula_scoped_in_world m
-        (denot_ty_lvar_gas (S gas) Σ (CTOver b φ) e2)).
+        (ty_denote_gas (S gas) Σ (CTOver b φ) e2)).
   {
     unfold formula_scoped_in_world.
-    eapply formula_fv_denot_ty_lvar_gas_scope_from_guard_pre_open;
+    eapply formula_fv_ty_denote_gas_scope_from_guard_pre_open;
       [reflexivity|exact Hguard_tgt].
   }
-  cbn [denot_ty_lvar_gas] in Hscope_tgt.
+  cbn [ty_denote_gas] in Hscope_tgt.
   pose proof (formula_scoped_and_r _ _ _ Hscope_tgt) as Hbody_scope.
   eapply res_models_forall_full_world_impl2_map;
     [exact Hbody_scope| |exact Hsrc].
@@ -58,13 +58,13 @@ Proof.
         | exact Hdom
         | exact Hrestrict
         | exact Hresult ].
-      eapply typed_total_tm_result_equiv_on_term_scope. exact Hequiv.
+      eapply typed_total_equiv_term_scope. exact Hequiv.
     + intros Hfib. exact Hfib.
 Qed.
 
-Lemma denot_ty_lvar_gas_tm_result_equiv_under_body
+Lemma ty_denote_gas_tm_equiv_under_body
     (gas : nat) (Σ : lty_env) b φ e1 e2 (m : WfWorldT) :
-  typed_total_tm_result_equiv_on Σ (CTUnder b φ) m e1 e2 ->
+  typed_total_equiv_on Σ (CTUnder b φ) m e1 e2 ->
   m ⊨
     FForall
       (FImpl (basic_world_formula (<[LVBound 0 := TBase b]> ∅))
@@ -81,21 +81,21 @@ Lemma denot_ty_lvar_gas_tm_result_equiv_under_body
             (FUnder (type_qualifier_formula φ))))).
 Proof.
   intros Hequiv Hsrc.
-  pose proof (typed_total_tm_result_equiv_on_term_lc_lvars
+  pose proof (typed_total_equiv_term_lc_lvars
     Σ (CTUnder b φ) m e1 e2 Hequiv) as [Hlc_e1 Hlc_e2].
-  pose proof (typed_total_tm_result_equiv_on_target_zero
+  pose proof (typed_total_equiv_target_zero
     Σ (CTUnder b φ) m e1 e2 Hequiv) as Hzero_tgt.
-  pose proof (denot_ty_lvar_gas_guard_of_zero
+  pose proof (ty_denote_gas_guard_of_zero
     Σ (CTUnder b φ) e2 m Hzero_tgt) as Hguard_tgt.
   assert (Hscope_tgt :
       formula_scoped_in_world m
-        (denot_ty_lvar_gas (S gas) Σ (CTUnder b φ) e2)).
+        (ty_denote_gas (S gas) Σ (CTUnder b φ) e2)).
   {
     unfold formula_scoped_in_world.
-    eapply formula_fv_denot_ty_lvar_gas_scope_from_guard_pre_open;
+    eapply formula_fv_ty_denote_gas_scope_from_guard_pre_open;
       [reflexivity|exact Hguard_tgt].
   }
-  cbn [denot_ty_lvar_gas] in Hscope_tgt.
+  cbn [ty_denote_gas] in Hscope_tgt.
   pose proof (formula_scoped_and_r _ _ _ Hscope_tgt) as Hbody_scope.
   eapply res_models_forall_full_world_impl2_map;
     [exact Hbody_scope| |exact Hsrc].
@@ -113,21 +113,21 @@ Proof.
         | exact Hdom
         | exact Hrestrict
         | exact Hresult ].
-      eapply typed_total_tm_result_equiv_on_term_scope. exact Hequiv.
+      eapply typed_total_equiv_term_scope. exact Hequiv.
     + intros Hfib. exact Hfib.
 Qed.
 
-Lemma denot_ty_lvar_gas_zero_project_context
+Lemma ty_denote_gas_zero_project_context
     (Σ : lty_env) τsmall τbig e (m : WfWorldT) :
   context_ty_lvars τsmall ⊆ context_ty_lvars τbig ->
   erase_ty τsmall = erase_ty τbig ->
   context_ty_shape_ok τsmall ->
-  m ⊨ denot_ty_lvar_gas 0 Σ τbig e ->
-  m ⊨ denot_ty_lvar_gas 0 Σ τsmall e.
+  m ⊨ ty_denote_gas 0 Σ τbig e ->
+  m ⊨ ty_denote_gas 0 Σ τsmall e.
 Proof.
   intros Hτ Herase Hshape_small Hzero.
-  apply denot_ty_lvar_gas_zero_of_guard.
-  apply denot_ty_lvar_gas_guard_of_zero in Hzero.
+  apply ty_denote_gas_zero_of_guard.
+  apply ty_denote_gas_guard_of_zero in Hzero.
   repeat rewrite res_models_and_iff in Hzero |- *.
   destruct Hzero as [Hwf [Hworld [Hbasic Htotal]]].
   pose proof (denot_relevant_env_dom_mono_context
@@ -188,31 +188,31 @@ Proof.
       * exact Htotal.
 Qed.
 
-Lemma denot_ty_lvar_gas_zero_inter_l
+Lemma ty_denote_gas_zero_inter_l
     (Σ : lty_env) τ1 τ2 e (m : WfWorldT) :
-  m ⊨ denot_ty_lvar_gas 0 Σ (CTInter τ1 τ2) e ->
-  m ⊨ denot_ty_lvar_gas 0 Σ τ1 e.
+  m ⊨ ty_denote_gas 0 Σ (CTInter τ1 τ2) e ->
+  m ⊨ ty_denote_gas 0 Σ τ1 e.
 Proof.
   intros Hzero.
-  eapply (denot_ty_lvar_gas_zero_project_context
+  eapply (ty_denote_gas_zero_project_context
     Σ τ1 (CTInter τ1 τ2) e m); [|reflexivity| |exact Hzero].
   - cbn [context_ty_lvars context_ty_lvars_at]. set_solver.
-  - apply denot_ty_lvar_gas_guard_of_zero in Hzero.
+  - apply ty_denote_gas_guard_of_zero in Hzero.
     repeat rewrite res_models_and_iff in Hzero.
     destruct Hzero as [Hwf _].
     apply context_ty_wf_formula_models_iff in Hwf as [_ [_ [_ Hshape]]].
     cbn [context_ty_shape_ok] in Hshape. tauto.
 Qed.
 
-Lemma denot_ty_lvar_gas_zero_inter_r
+Lemma ty_denote_gas_zero_inter_r
     (Σ : lty_env) τ1 τ2 e (m : WfWorldT) :
-  m ⊨ denot_ty_lvar_gas 0 Σ (CTInter τ1 τ2) e ->
-  m ⊨ denot_ty_lvar_gas 0 Σ τ2 e.
+  m ⊨ ty_denote_gas 0 Σ (CTInter τ1 τ2) e ->
+  m ⊨ ty_denote_gas 0 Σ τ2 e.
 Proof.
   intros Hzero.
   assert (Hshape_big : context_ty_shape_ok (CTInter τ1 τ2)).
   {
-    apply denot_ty_lvar_gas_guard_of_zero in Hzero as Hguard.
+    apply ty_denote_gas_guard_of_zero in Hzero as Hguard.
     repeat rewrite res_models_and_iff in Hguard.
     destruct Hguard as [Hwf _].
     apply context_ty_wf_formula_models_iff in Hwf as [_ [_ [_ Hshape]]].
@@ -220,81 +220,81 @@ Proof.
   }
   cbn [context_ty_shape_ok] in Hshape_big.
   destruct Hshape_big as [_ [Hshape2 Herase]].
-  eapply (denot_ty_lvar_gas_zero_project_context
+  eapply (ty_denote_gas_zero_project_context
     Σ τ2 (CTInter τ1 τ2) e m); [| |exact Hshape2|exact Hzero].
   - cbn [context_ty_lvars context_ty_lvars_at]. set_solver.
   - cbn [erase_ty]. symmetry. exact Herase.
 Qed.
 
-Lemma typed_total_tm_result_equiv_on_inter_l
+Lemma typed_total_equiv_inter_l
     (Σ : lty_env) τ1 τ2 m e1 e2 :
-  typed_total_tm_result_equiv_on Σ (CTInter τ1 τ2) m e1 e2 ->
-  typed_total_tm_result_equiv_on Σ τ1 m e1 e2.
+  typed_total_equiv_on Σ (CTInter τ1 τ2) m e1 e2 ->
+  typed_total_equiv_on Σ τ1 m e1 e2.
 Proof.
   intros [Heq [Hzero_src Hzero_tgt]].
   split; [exact Heq|].
   split.
-  - eapply denot_ty_lvar_gas_zero_inter_l; exact Hzero_src.
-  - eapply denot_ty_lvar_gas_zero_inter_l; exact Hzero_tgt.
+  - eapply ty_denote_gas_zero_inter_l; exact Hzero_src.
+  - eapply ty_denote_gas_zero_inter_l; exact Hzero_tgt.
 Qed.
 
-Lemma typed_total_tm_result_equiv_on_inter_r
+Lemma typed_total_equiv_inter_r
     (Σ : lty_env) τ1 τ2 m e1 e2 :
-  typed_total_tm_result_equiv_on Σ (CTInter τ1 τ2) m e1 e2 ->
-  typed_total_tm_result_equiv_on Σ τ2 m e1 e2.
+  typed_total_equiv_on Σ (CTInter τ1 τ2) m e1 e2 ->
+  typed_total_equiv_on Σ τ2 m e1 e2.
 Proof.
   intros [Heq [Hzero_src Hzero_tgt]].
   split; [exact Heq|].
   split.
-  - eapply denot_ty_lvar_gas_zero_inter_r; exact Hzero_src.
-  - eapply denot_ty_lvar_gas_zero_inter_r; exact Hzero_tgt.
+  - eapply ty_denote_gas_zero_inter_r; exact Hzero_src.
+  - eapply ty_denote_gas_zero_inter_r; exact Hzero_tgt.
 Qed.
 
-Lemma denot_ty_lvar_gas_tm_result_equiv_inter_body
+Lemma ty_denote_gas_tm_equiv_inter_body
     gas (IH : forall Σ τ e1 e2 (m : WfWorldT),
-      typed_total_tm_result_equiv_on Σ τ m e1 e2 ->
-      m ⊨ denot_ty_lvar_gas gas Σ τ e1 ->
-      m ⊨ denot_ty_lvar_gas gas Σ τ e2)
+      typed_total_equiv_on Σ τ m e1 e2 ->
+      m ⊨ ty_denote_gas gas Σ τ e1 ->
+      m ⊨ ty_denote_gas gas Σ τ e2)
     (Σ : lty_env) τ1 τ2 e1 e2 (m : WfWorldT) :
-  typed_total_tm_result_equiv_on Σ (CTInter τ1 τ2) m e1 e2 ->
-  m ⊨ denot_ty_lvar_gas gas Σ τ1 e1 /\
-  m ⊨ denot_ty_lvar_gas gas Σ τ2 e1 ->
-  m ⊨ denot_ty_lvar_gas gas Σ τ1 e2 /\
-  m ⊨ denot_ty_lvar_gas gas Σ τ2 e2.
+  typed_total_equiv_on Σ (CTInter τ1 τ2) m e1 e2 ->
+  m ⊨ ty_denote_gas gas Σ τ1 e1 /\
+  m ⊨ ty_denote_gas gas Σ τ2 e1 ->
+  m ⊨ ty_denote_gas gas Σ τ1 e2 /\
+  m ⊨ ty_denote_gas gas Σ τ2 e2.
 Proof.
   intros Hequiv [H1 H2].
   split.
   - eapply IH; [|exact H1].
-    eapply typed_total_tm_result_equiv_on_inter_l; exact Hequiv.
+    eapply typed_total_equiv_inter_l; exact Hequiv.
   - eapply IH; [|exact H2].
-    eapply typed_total_tm_result_equiv_on_inter_r; exact Hequiv.
+    eapply typed_total_equiv_inter_r; exact Hequiv.
 Qed.
 
-Lemma denot_ty_lvar_gas_zero_union_l
+Lemma ty_denote_gas_zero_union_l
     (Σ : lty_env) τ1 τ2 e (m : WfWorldT) :
-  m ⊨ denot_ty_lvar_gas 0 Σ (CTUnion τ1 τ2) e ->
-  m ⊨ denot_ty_lvar_gas 0 Σ τ1 e.
+  m ⊨ ty_denote_gas 0 Σ (CTUnion τ1 τ2) e ->
+  m ⊨ ty_denote_gas 0 Σ τ1 e.
 Proof.
   intros Hzero.
-  eapply (denot_ty_lvar_gas_zero_project_context
+  eapply (ty_denote_gas_zero_project_context
     Σ τ1 (CTUnion τ1 τ2) e m); [|reflexivity| |exact Hzero].
   - cbn [context_ty_lvars context_ty_lvars_at]. set_solver.
-  - apply denot_ty_lvar_gas_guard_of_zero in Hzero.
+  - apply ty_denote_gas_guard_of_zero in Hzero.
     repeat rewrite res_models_and_iff in Hzero.
     destruct Hzero as [Hwf _].
     apply context_ty_wf_formula_models_iff in Hwf as [_ [_ [_ Hshape]]].
     cbn [context_ty_shape_ok] in Hshape. tauto.
 Qed.
 
-Lemma denot_ty_lvar_gas_zero_union_r
+Lemma ty_denote_gas_zero_union_r
     (Σ : lty_env) τ1 τ2 e (m : WfWorldT) :
-  m ⊨ denot_ty_lvar_gas 0 Σ (CTUnion τ1 τ2) e ->
-  m ⊨ denot_ty_lvar_gas 0 Σ τ2 e.
+  m ⊨ ty_denote_gas 0 Σ (CTUnion τ1 τ2) e ->
+  m ⊨ ty_denote_gas 0 Σ τ2 e.
 Proof.
   intros Hzero.
   assert (Hshape_big : context_ty_shape_ok (CTUnion τ1 τ2)).
   {
-    apply denot_ty_lvar_gas_guard_of_zero in Hzero as Hguard.
+    apply ty_denote_gas_guard_of_zero in Hzero as Hguard.
     repeat rewrite res_models_and_iff in Hguard.
     destruct Hguard as [Hwf _].
     apply context_ty_wf_formula_models_iff in Hwf as [_ [_ [_ Hshape]]].
@@ -302,92 +302,92 @@ Proof.
   }
   cbn [context_ty_shape_ok] in Hshape_big.
   destruct Hshape_big as [_ [Hshape2 Herase]].
-  eapply (denot_ty_lvar_gas_zero_project_context
+  eapply (ty_denote_gas_zero_project_context
     Σ τ2 (CTUnion τ1 τ2) e m); [| |exact Hshape2|exact Hzero].
   - cbn [context_ty_lvars context_ty_lvars_at]. set_solver.
   - cbn [erase_ty]. symmetry. exact Herase.
 Qed.
 
-Lemma typed_total_tm_result_equiv_on_union_l
+Lemma typed_total_equiv_union_l
     (Σ : lty_env) τ1 τ2 m e1 e2 :
-  typed_total_tm_result_equiv_on Σ (CTUnion τ1 τ2) m e1 e2 ->
-  typed_total_tm_result_equiv_on Σ τ1 m e1 e2.
+  typed_total_equiv_on Σ (CTUnion τ1 τ2) m e1 e2 ->
+  typed_total_equiv_on Σ τ1 m e1 e2.
 Proof.
   intros [Heq [Hzero_src Hzero_tgt]].
   split; [exact Heq|].
   split.
-  - eapply denot_ty_lvar_gas_zero_union_l; exact Hzero_src.
-  - eapply denot_ty_lvar_gas_zero_union_l; exact Hzero_tgt.
+  - eapply ty_denote_gas_zero_union_l; exact Hzero_src.
+  - eapply ty_denote_gas_zero_union_l; exact Hzero_tgt.
 Qed.
 
-Lemma typed_total_tm_result_equiv_on_union_r
+Lemma typed_total_equiv_union_r
     (Σ : lty_env) τ1 τ2 m e1 e2 :
-  typed_total_tm_result_equiv_on Σ (CTUnion τ1 τ2) m e1 e2 ->
-  typed_total_tm_result_equiv_on Σ τ2 m e1 e2.
+  typed_total_equiv_on Σ (CTUnion τ1 τ2) m e1 e2 ->
+  typed_total_equiv_on Σ τ2 m e1 e2.
 Proof.
   intros [Heq [Hzero_src Hzero_tgt]].
   split; [exact Heq|].
   split.
-  - eapply denot_ty_lvar_gas_zero_union_r; exact Hzero_src.
-  - eapply denot_ty_lvar_gas_zero_union_r; exact Hzero_tgt.
+  - eapply ty_denote_gas_zero_union_r; exact Hzero_src.
+  - eapply ty_denote_gas_zero_union_r; exact Hzero_tgt.
 Qed.
 
-Lemma denot_ty_lvar_gas_scope_from_zero_any
+Lemma ty_denote_gas_scope_from_zero_any
     gas Σ τ e (m : WfWorldT) :
-  m ⊨ denot_ty_lvar_gas 0 Σ τ e ->
-  formula_scoped_in_world m (denot_ty_lvar_gas gas Σ τ e).
+  m ⊨ ty_denote_gas 0 Σ τ e ->
+  formula_scoped_in_world m (ty_denote_gas gas Σ τ e).
 Proof.
   intros Hzero.
-  eapply formula_fv_denot_ty_lvar_gas_scope_from_guard_pre_open.
+  eapply formula_fv_ty_denote_gas_scope_from_guard_pre_open.
   - reflexivity.
-  - apply denot_ty_lvar_gas_guard_of_zero. exact Hzero.
+  - apply ty_denote_gas_guard_of_zero. exact Hzero.
 Qed.
 
-Lemma denot_ty_lvar_gas_tm_result_equiv_union_body
+Lemma ty_denote_gas_tm_equiv_union_body
     gas (IH : forall Σ τ e1 e2 (m : WfWorldT),
-      typed_total_tm_result_equiv_on Σ τ m e1 e2 ->
-      m ⊨ denot_ty_lvar_gas gas Σ τ e1 ->
-      m ⊨ denot_ty_lvar_gas gas Σ τ e2)
+      typed_total_equiv_on Σ τ m e1 e2 ->
+      m ⊨ ty_denote_gas gas Σ τ e1 ->
+      m ⊨ ty_denote_gas gas Σ τ e2)
     (Σ : lty_env) τ1 τ2 e1 e2 (m : WfWorldT) :
-  typed_total_tm_result_equiv_on Σ (CTUnion τ1 τ2) m e1 e2 ->
+  typed_total_equiv_on Σ (CTUnion τ1 τ2) m e1 e2 ->
   m ⊨
     FOr
-      (denot_ty_lvar_gas gas Σ τ1 e1)
-      (denot_ty_lvar_gas gas Σ τ2 e1) ->
+      (ty_denote_gas gas Σ τ1 e1)
+      (ty_denote_gas gas Σ τ2 e1) ->
   m ⊨
     FOr
-	      (denot_ty_lvar_gas gas Σ τ1 e2)
-	      (denot_ty_lvar_gas gas Σ τ2 e2).
+	      (ty_denote_gas gas Σ τ1 e2)
+	      (ty_denote_gas gas Σ τ2 e2).
 Proof.
   intros Hequiv Hbody.
-  pose proof (typed_total_tm_result_equiv_on_union_l
+  pose proof (typed_total_equiv_union_l
     Σ τ1 τ2 m e1 e2 Hequiv) as Hequiv1.
-  pose proof (typed_total_tm_result_equiv_on_union_r
+  pose proof (typed_total_equiv_union_r
     Σ τ1 τ2 m e1 e2 Hequiv) as Hequiv2.
   pose proof (res_models_scoped _ _ Hbody) as Hscope_body.
   apply (proj1 (res_models_or_iff m _ _ Hscope_body)) in Hbody.
   destruct Hbody as [H1|H2].
   - eapply res_models_or_intro_l_from_model.
     + eapply IH; [exact Hequiv1|exact H1].
-    + eapply denot_ty_lvar_gas_scope_from_zero_any.
-      exact (typed_total_tm_result_equiv_on_target_zero
+    + eapply ty_denote_gas_scope_from_zero_any.
+      exact (typed_total_equiv_target_zero
         Σ τ2 m e1 e2 Hequiv2).
   - eapply res_models_or_intro_r_from_model.
-    + eapply denot_ty_lvar_gas_scope_from_zero_any.
-      exact (typed_total_tm_result_equiv_on_target_zero
+    + eapply ty_denote_gas_scope_from_zero_any.
+      exact (typed_total_equiv_target_zero
         Σ τ1 m e1 e2 Hequiv1).
     + eapply IH; [exact Hequiv2|exact H2].
 Qed.
 
-Lemma denot_ty_lvar_gas_zero_res_subset
+Lemma ty_denote_gas_zero_res_subset
     (Σ : lty_env) τ e (m n : WfWorldT) :
   res_subset n m ->
-  m ⊨ denot_ty_lvar_gas 0 Σ τ e ->
-  n ⊨ denot_ty_lvar_gas 0 Σ τ e.
+  m ⊨ ty_denote_gas 0 Σ τ e ->
+  n ⊨ ty_denote_gas 0 Σ τ e.
 Proof.
   intros Hsub Hzero.
-  apply denot_ty_lvar_gas_zero_of_guard.
-  apply denot_ty_lvar_gas_guard_of_zero in Hzero.
+  apply ty_denote_gas_zero_of_guard.
+  apply ty_denote_gas_guard_of_zero in Hzero.
   repeat rewrite res_models_and_iff in Hzero |- *.
   destruct Hzero as [Hwf [Hworld [Hbasic Htotal]]].
   pose proof Hsub as [Hdom _].
@@ -405,31 +405,31 @@ Proof.
       * eapply expr_total_formula_res_subset; eauto.
 Qed.
 
-Lemma denot_ty_lvar_gas_zero_sum_l
+Lemma ty_denote_gas_zero_sum_l
     (Σ : lty_env) τ1 τ2 e (m : WfWorldT) :
-  m ⊨ denot_ty_lvar_gas 0 Σ (CTSum τ1 τ2) e ->
-  m ⊨ denot_ty_lvar_gas 0 Σ τ1 e.
+  m ⊨ ty_denote_gas 0 Σ (CTSum τ1 τ2) e ->
+  m ⊨ ty_denote_gas 0 Σ τ1 e.
 Proof.
   intros Hzero.
-  eapply (denot_ty_lvar_gas_zero_project_context
+  eapply (ty_denote_gas_zero_project_context
     Σ τ1 (CTSum τ1 τ2) e m); [|reflexivity| |exact Hzero].
   - cbn [context_ty_lvars context_ty_lvars_at]. set_solver.
-  - apply denot_ty_lvar_gas_guard_of_zero in Hzero.
+  - apply ty_denote_gas_guard_of_zero in Hzero.
     repeat rewrite res_models_and_iff in Hzero.
     destruct Hzero as [Hwf _].
     apply context_ty_wf_formula_models_iff in Hwf as [_ [_ [_ Hshape]]].
     cbn [context_ty_shape_ok] in Hshape. tauto.
 Qed.
 
-Lemma denot_ty_lvar_gas_zero_sum_r
+Lemma ty_denote_gas_zero_sum_r
     (Σ : lty_env) τ1 τ2 e (m : WfWorldT) :
-  m ⊨ denot_ty_lvar_gas 0 Σ (CTSum τ1 τ2) e ->
-  m ⊨ denot_ty_lvar_gas 0 Σ τ2 e.
+  m ⊨ ty_denote_gas 0 Σ (CTSum τ1 τ2) e ->
+  m ⊨ ty_denote_gas 0 Σ τ2 e.
 Proof.
   intros Hzero.
   assert (Hshape_big : context_ty_shape_ok (CTSum τ1 τ2)).
   {
-    apply denot_ty_lvar_gas_guard_of_zero in Hzero as Hguard.
+    apply ty_denote_gas_guard_of_zero in Hzero as Hguard.
     repeat rewrite res_models_and_iff in Hguard.
     destruct Hguard as [Hwf _].
     apply context_ty_wf_formula_models_iff in Hwf as [_ [_ [_ Hshape]]].
@@ -437,83 +437,83 @@ Proof.
   }
   cbn [context_ty_shape_ok] in Hshape_big.
   destruct Hshape_big as [_ [Hshape2 Herase]].
-  eapply (denot_ty_lvar_gas_zero_project_context
+  eapply (ty_denote_gas_zero_project_context
     Σ τ2 (CTSum τ1 τ2) e m); [| |exact Hshape2|exact Hzero].
   - cbn [context_ty_lvars context_ty_lvars_at]. set_solver.
   - cbn [erase_ty]. symmetry. exact Herase.
 Qed.
 
-Lemma typed_total_tm_result_equiv_on_sum_l_target_zero
+Lemma typed_total_equiv_sum_l_target_zero
     (Σ : lty_env) τ1 τ2 (e1 e2 : tm) (m m1 : WfWorldT) :
   res_subset m1 m ->
-  m ⊨ denot_ty_lvar_gas 0 Σ (CTSum τ1 τ2) e2 ->
-  m1 ⊨ denot_ty_lvar_gas 0 Σ τ1 e2.
+  m ⊨ ty_denote_gas 0 Σ (CTSum τ1 τ2) e2 ->
+  m1 ⊨ ty_denote_gas 0 Σ τ1 e2.
 Proof.
   intros Hsub Hzero.
-  apply denot_ty_lvar_gas_zero_sum_l with (τ2 := τ2).
-  eapply denot_ty_lvar_gas_zero_res_subset; eauto.
+  apply ty_denote_gas_zero_sum_l with (τ2 := τ2).
+  eapply ty_denote_gas_zero_res_subset; eauto.
 Qed.
 
-Lemma typed_total_tm_result_equiv_on_sum_r_target_zero
+Lemma typed_total_equiv_sum_r_target_zero
     (Σ : lty_env) τ1 τ2 (e1 e2 : tm) (m m2 : WfWorldT) :
   res_subset m2 m ->
-  m ⊨ denot_ty_lvar_gas 0 Σ (CTSum τ1 τ2) e2 ->
-  m2 ⊨ denot_ty_lvar_gas 0 Σ τ2 e2.
+  m ⊨ ty_denote_gas 0 Σ (CTSum τ1 τ2) e2 ->
+  m2 ⊨ ty_denote_gas 0 Σ τ2 e2.
 Proof.
   intros Hsub Hzero.
-  apply denot_ty_lvar_gas_zero_sum_r with (τ1 := τ1).
-  eapply denot_ty_lvar_gas_zero_res_subset; eauto.
+  apply ty_denote_gas_zero_sum_r with (τ1 := τ1).
+  eapply ty_denote_gas_zero_res_subset; eauto.
 Qed.
 
-Lemma typed_total_tm_result_equiv_on_sum_l_pullback
+Lemma typed_total_equiv_sum_l_pullback
     gas (Σ : lty_env) τ1 τ2 e1 e2 (m m1 : WfWorldT) :
   res_subset m1 m ->
-  typed_total_tm_result_equiv_on Σ (CTSum τ1 τ2) m e1 e2 ->
-  m1 ⊨ denot_ty_lvar_gas gas Σ τ1 e1 ->
-  typed_total_tm_result_equiv_on Σ τ1 m1 e1 e2.
+  typed_total_equiv_on Σ (CTSum τ1 τ2) m e1 e2 ->
+  m1 ⊨ ty_denote_gas gas Σ τ1 e1 ->
+  typed_total_equiv_on Σ τ1 m1 e1 e2.
 Proof.
   intros Hsub [Heq [_ Hzero_tgt]] Hsrc.
   split.
-  - eapply tm_result_equiv_on_res_store_subset; eauto.
+  - eapply tm_equiv_res_store_subset; eauto.
   - split.
-    + apply denot_ty_lvar_gas_zero_of_guard.
-      eapply denot_ty_lvar_gas_guard. exact Hsrc.
-    + eapply typed_total_tm_result_equiv_on_sum_l_target_zero;
+    + apply ty_denote_gas_zero_of_guard.
+      eapply ty_denote_gas_guard. exact Hsrc.
+    + eapply typed_total_equiv_sum_l_target_zero;
         eauto.
 Qed.
 
-Lemma typed_total_tm_result_equiv_on_sum_r_pullback
+Lemma typed_total_equiv_sum_r_pullback
     gas (Σ : lty_env) τ1 τ2 e1 e2 (m m2 : WfWorldT) :
   res_subset m2 m ->
-  typed_total_tm_result_equiv_on Σ (CTSum τ1 τ2) m e1 e2 ->
-  m2 ⊨ denot_ty_lvar_gas gas Σ τ2 e1 ->
-  typed_total_tm_result_equiv_on Σ τ2 m2 e1 e2.
+  typed_total_equiv_on Σ (CTSum τ1 τ2) m e1 e2 ->
+  m2 ⊨ ty_denote_gas gas Σ τ2 e1 ->
+  typed_total_equiv_on Σ τ2 m2 e1 e2.
 Proof.
   intros Hsub [Heq [_ Hzero_tgt]] Hsrc.
   split.
-  - eapply tm_result_equiv_on_res_store_subset; eauto.
+  - eapply tm_equiv_res_store_subset; eauto.
   - split.
-    + apply denot_ty_lvar_gas_zero_of_guard.
-      eapply denot_ty_lvar_gas_guard. exact Hsrc.
-    + eapply typed_total_tm_result_equiv_on_sum_r_target_zero;
+    + apply ty_denote_gas_zero_of_guard.
+      eapply ty_denote_gas_guard. exact Hsrc.
+    + eapply typed_total_equiv_sum_r_target_zero;
         eauto.
 Qed.
 
-Lemma denot_ty_lvar_gas_tm_result_equiv_sum_body
+Lemma ty_denote_gas_tm_equiv_sum_body
     gas (IH : forall Σ τ e1 e2 (m : WfWorldT),
-      typed_total_tm_result_equiv_on Σ τ m e1 e2 ->
-      m ⊨ denot_ty_lvar_gas gas Σ τ e1 ->
-      m ⊨ denot_ty_lvar_gas gas Σ τ e2)
+      typed_total_equiv_on Σ τ m e1 e2 ->
+      m ⊨ ty_denote_gas gas Σ τ e1 ->
+      m ⊨ ty_denote_gas gas Σ τ e2)
     (Σ : lty_env) τ1 τ2 e1 e2 (m : WfWorldT) :
-  typed_total_tm_result_equiv_on Σ (CTSum τ1 τ2) m e1 e2 ->
+  typed_total_equiv_on Σ (CTSum τ1 τ2) m e1 e2 ->
   m ⊨
     FPlus
-      (denot_ty_lvar_gas gas Σ τ1 e1)
-      (denot_ty_lvar_gas gas Σ τ2 e1) ->
+      (ty_denote_gas gas Σ τ1 e1)
+      (ty_denote_gas gas Σ τ2 e1) ->
   m ⊨
     FPlus
-	      (denot_ty_lvar_gas gas Σ τ1 e2)
-	      (denot_ty_lvar_gas gas Σ τ2 e2).
+	      (ty_denote_gas gas Σ τ1 e2)
+	      (ty_denote_gas gas Σ τ2 e2).
 Proof.
   intros Hequiv Hbody.
   apply res_models_plus_iff in Hbody as
@@ -522,25 +522,25 @@ Proof.
     as [Hsub1 [Hsub2 [Hdef_full Hle_full]]].
   set (m1 := res_pullback_subset_projection m n1 Hsub1).
   set (m2 := res_pullback_subset_projection m n2 Hsub2).
-  assert (Hτ1_full : m1 ⊨ denot_ty_lvar_gas gas Σ τ1 e1).
+  assert (Hτ1_full : m1 ⊨ ty_denote_gas gas Σ τ1 e1).
   {
     subst m1.
     eapply res_models_pullback_subset_projection. exact Hτ1.
   }
-  assert (Hτ2_full : m2 ⊨ denot_ty_lvar_gas gas Σ τ2 e1).
+  assert (Hτ2_full : m2 ⊨ ty_denote_gas gas Σ τ2 e1).
   {
     subst m2.
     eapply res_models_pullback_subset_projection. exact Hτ2.
   }
 	  eapply res_models_plus_intro; [exact Hle_full| |].
 	  - eapply IH; [|exact Hτ1_full].
-	    refine (typed_total_tm_result_equiv_on_sum_l_pullback
+	    refine (typed_total_equiv_sum_l_pullback
 	      gas Σ τ1 τ2 e1 e2 m m1 _ Hequiv Hτ1_full).
 	    subst m1. apply res_pullback_subset_projection_subset.
 	  - eapply IH; [|exact Hτ2_full].
-	    refine (typed_total_tm_result_equiv_on_sum_r_pullback
+	    refine (typed_total_equiv_sum_r_pullback
 	      gas Σ τ1 τ2 e1 e2 m m2 _ Hequiv Hτ2_full).
 	    subst m2. apply res_pullback_subset_projection_subset.
 	Qed.
 
-End ContextTypeDenotation.
+End TypeDenote.
