Denotation/theories/TypeEquivWand.v
@@ -1,37 +1,38 @@
-(** * Denotation.ContextTypeDenotationSaturateArrow
+(** * Denotation.TypeEquivWand
 
-    Arrow case for term-result-equivalence transport. *)
+    Wand case for term-result-equivalence transport. *)
 
-From Denotation Require Import Notation ContextTypeDenotationOpen.
+From Denotation Require Import Notation TypeDenoteOpen.
 From Denotation Require Import
-  ContextTypeDenotationSaturateCore
-  ContextTypeDenotationSaturateBody.
+  TypeEquivCore
+  TypeEquivBody
+  TypeEquivArrow.
 
-Section ContextTypeDenotation.
+Section TypeDenote.
 
-Lemma denot_ty_lvar_gas_tm_result_equiv_arrow_open_arg
+Lemma ty_denote_gas_tm_equiv_wand_open_arg
     gas (Σ : lty_env) τx τr e1 e2
-    (m my : WfWorldT) y :
-  typed_total_tm_result_equiv_on Σ (CTArrow τx τr) m e1 e2 ->
+    (m my n : WfWorldT) y (Hc : world_compat n my) :
+  typed_total_equiv_on Σ (CTWand τx τr) m e1 e2 ->
   world_dom (my : WorldT) = world_dom (m : WorldT) ∪ {[y]} ->
   res_restrict my (world_dom (m : WorldT)) = m ->
   y ∉ fv_cty τx ->
   y ∉ lvars_fv
     (dom (typed_lty_env_bind
-      (denot_relevant_env Σ (CTArrow τx τr) e1) (erase_ty τx))) ->
+      (denot_relevant_env Σ (CTWand τx τr) e1) (erase_ty τx))) ->
   y ∉ lvars_fv
     (dom (typed_lty_env_bind
-      (denot_relevant_env Σ (CTArrow τx τr) e2) (erase_ty τx))) ->
-  my ⊨ formula_open 0 y
-    (denot_ty_lvar_gas gas
+      (denot_relevant_env Σ (CTWand τx τr) e2) (erase_ty τx))) ->
+  n ⊨ formula_open 0 y
+    (ty_denote_gas gas
       (typed_lty_env_bind
-        (denot_relevant_env Σ (CTArrow τx τr) e2)
+        (denot_relevant_env Σ (CTWand τx τr) e2)
         (erase_ty τx))
       (cty_shift 0 τx) (tret (vbvar 0))) ->
-  my ⊨ formula_open 0 y
-    (denot_ty_lvar_gas gas
+  n ⊨ formula_open 0 y
+    (ty_denote_gas gas
       (typed_lty_env_bind
-        (denot_relevant_env Σ (CTArrow τx τr) e1)
+        (denot_relevant_env Σ (CTWand τx τr) e1)
         (erase_ty τx))
       (cty_shift 0 τx) (tret (vbvar 0))).
 Proof.
@@ -40,14 +41,14 @@ Proof.
   { rewrite cty_shift_fv. exact Hyτx. }
   assert (Hea_fresh : y ∉ fv_tm (tret (vbvar 0))).
   { cbn [fv_tm fv_value]. set_solver. }
-  rewrite (formula_open_denot_ty_lvar_gas_singleton 0 y gas
+  rewrite (formula_open_ty_denote_gas_singleton 0 y gas
     (typed_lty_env_bind
-      (denot_relevant_env Σ (CTArrow τx τr) e2) (erase_ty τx))
+      (denot_relevant_env Σ (CTWand τx τr) e2) (erase_ty τx))
     (cty_shift 0 τx) (tret (vbvar 0))) in Htgt
     by (exact HyΣ2 || exact Hea_fresh || exact Hτa_fresh).
-  rewrite (formula_open_denot_ty_lvar_gas_singleton 0 y gas
+  rewrite (formula_open_ty_denote_gas_singleton 0 y gas
     (typed_lty_env_bind
-      (denot_relevant_env Σ (CTArrow τx τr) e1) (erase_ty τx))
+      (denot_relevant_env Σ (CTWand τx τr) e1) (erase_ty τx))
     (cty_shift 0 τx) (tret (vbvar 0)))
     by (exact HyΣ1 || exact Hea_fresh || exact Hτa_fresh).
   replace (open_tm 0 (vfvar y) (tret (vbvar 0))) with
@@ -56,56 +57,56 @@ Proof.
   set (τa := cty_open 0 y (cty_shift 0 τx)).
   set (ea := tret (vfvar y)).
   fold τa ea in Htgt |- *.
-  pose proof (denot_ty_lvar_gas_env_agree_on gas
+  pose proof (ty_denote_gas_env_agree_on gas
     (lty_env_open_one 0 y
       (typed_lty_env_bind
-        (denot_relevant_env Σ (CTArrow τx τr) e1) (erase_ty τx)))
+        (denot_relevant_env Σ (CTWand τx τr) e1) (erase_ty τx)))
     (lty_env_open_one 0 y (typed_lty_env_bind Σ (erase_ty τx)))
     τa ea (denot_relevant_lvars τa ea)
     ltac:(set_solver)
-    (arrow_arg_relevant_env_agree_open_one_core
+    (wand_arg_relevant_env_agree_open_one_core
       Σ (erase_ty τx) y τx τr e1 Hyτx)) as Hsrc_mid.
-  pose proof (denot_ty_lvar_gas_env_agree_on gas
+  pose proof (ty_denote_gas_env_agree_on gas
     (lty_env_open_one 0 y
       (typed_lty_env_bind
-        (denot_relevant_env Σ (CTArrow τx τr) e2) (erase_ty τx)))
+        (denot_relevant_env Σ (CTWand τx τr) e2) (erase_ty τx)))
     (lty_env_open_one 0 y (typed_lty_env_bind Σ (erase_ty τx)))
     τa ea (denot_relevant_lvars τa ea)
     ltac:(set_solver)
-    (arrow_arg_relevant_env_agree_open_one_core
+    (wand_arg_relevant_env_agree_open_one_core
       Σ (erase_ty τx) y τx τr e2 Hyτx)) as Htgt_mid.
   rewrite Hsrc_mid.
   rewrite Htgt_mid in Htgt.
   exact Htgt.
 Qed.
 
-Lemma denot_ty_lvar_gas_tm_result_equiv_arrow_open_result_source_mid
+Lemma ty_denote_gas_tm_equiv_wand_open_result_source_mid
     gas (Σ : lty_env) τx τr e1
-    (my : WfWorldT) y :
+    (m : WfWorldT) y :
   lc_tm e1 ->
   y ∉ fv_cty τr ->
-  my ⊨ denot_ty_lvar_gas gas
+  m ⊨ ty_denote_gas gas
     (lty_env_open_one 0 y
       (typed_lty_env_bind
-        (denot_relevant_env Σ (CTArrow τx τr) e1)
+        (denot_relevant_env Σ (CTWand τx τr) e1)
         (erase_ty τx)))
     (cty_open 0 y τr) (tapp_tm e1 (vfvar y)) ->
-  my ⊨ denot_ty_lvar_gas gas
+  m ⊨ ty_denote_gas gas
     (lty_env_open_one 0 y (typed_lty_env_bind Σ (erase_ty τx)))
     (cty_open 0 y τr) (tapp_tm e1 (vfvar y)).
 Proof.
   intros Hlc Hyτr Hsrc.
-  pose proof (denot_ty_lvar_gas_env_agree_on gas
+  pose proof (ty_denote_gas_env_agree_on gas
     (lty_env_open_one 0 y
       (typed_lty_env_bind
-        (denot_relevant_env Σ (CTArrow τx τr) e1)
+        (denot_relevant_env Σ (CTWand τx τr) e1)
         (erase_ty τx)))
     (lty_env_open_one 0 y (typed_lty_env_bind Σ (erase_ty τx)))
     (cty_open 0 y τr) (tapp_tm e1 (vfvar y))
     (denot_relevant_lvars (cty_open 0 y τr)
       (tapp_tm e1 (vfvar y)))
     ltac:(set_solver)
-    (arrow_body_relevant_env_agree_open_one_core
+    (wand_body_relevant_env_agree_open_one_core
       Σ (erase_ty τx) y τx τr e1 (tapp_tm e1 (vfvar y))
       Hyτr (tm_lvars_tapp_tm_fvar_without_arg_shift_lc e1 y Hlc)))
     as Hagree.
@@ -113,33 +114,33 @@ Proof.
   exact Hsrc.
 Qed.
 
-Lemma denot_ty_lvar_gas_tm_result_equiv_arrow_open_result_target_mid_to_goal
+Lemma ty_denote_gas_tm_equiv_wand_open_result_target_mid_to_goal
     gas (Σ : lty_env) τx τr e2
-    (my : WfWorldT) y :
+    (m : WfWorldT) y :
   lc_tm e2 ->
   y ∉ fv_cty τr ->
-  my ⊨ denot_ty_lvar_gas gas
+  m ⊨ ty_denote_gas gas
     (lty_env_open_one 0 y (typed_lty_env_bind Σ (erase_ty τx)))
     (cty_open 0 y τr) (tapp_tm e2 (vfvar y)) ->
-  my ⊨ denot_ty_lvar_gas gas
+  m ⊨ ty_denote_gas gas
     (lty_env_open_one 0 y
       (typed_lty_env_bind
-        (denot_relevant_env Σ (CTArrow τx τr) e2)
+        (denot_relevant_env Σ (CTWand τx τr) e2)
         (erase_ty τx)))
     (cty_open 0 y τr) (tapp_tm e2 (vfvar y)).
 Proof.
   intros Hlc Hyτr Hmid.
-  pose proof (denot_ty_lvar_gas_env_agree_on gas
+  pose proof (ty_denote_gas_env_agree_on gas
     (lty_env_open_one 0 y
       (typed_lty_env_bind
-        (denot_relevant_env Σ (CTArrow τx τr) e2)
+        (denot_relevant_env Σ (CTWand τx τr) e2)
         (erase_ty τx)))
     (lty_env_open_one 0 y (typed_lty_env_bind Σ (erase_ty τx)))
     (cty_open 0 y τr) (tapp_tm e2 (vfvar y))
     (denot_relevant_lvars (cty_open 0 y τr)
       (tapp_tm e2 (vfvar y)))
     ltac:(set_solver)
-    (arrow_body_relevant_env_agree_open_one_core
+    (wand_body_relevant_env_agree_open_one_core
       Σ (erase_ty τx) y τx τr e2 (tapp_tm e2 (vfvar y))
       Hyτr (tm_lvars_tapp_tm_fvar_without_arg_shift_lc e2 y Hlc)))
     as Hagree.
@@ -147,27 +148,28 @@ Proof.
   exact Hmid.
 Qed.
 
-Lemma wfworld_closed_on_arrow_open_result_apps
+Lemma wfworld_closed_on_wand_open_result_apps
     (Σ : lty_env) τx τr e1 e2
-    (m my : WfWorldT) y :
-  typed_total_tm_result_equiv_on Σ (CTArrow τx τr) m e1 e2 ->
+    (m my n : WfWorldT) y (Hc : world_compat n my) :
+  typed_total_equiv_on Σ (CTWand τx τr) m e1 e2 ->
   world_dom (my : WorldT) = world_dom (m : WorldT) ∪ {[y]} ->
   res_restrict my (world_dom (m : WorldT)) = m ->
   my ⊨ formula_open 0 y
     (basic_world_formula (<[LVBound 0 := erase_ty τx]> ∅)) ->
   wfworld_closed_on
     (fv_tm (tapp_tm e1 (vfvar y)) ∪
-     fv_tm (tapp_tm e2 (vfvar y))) my.
+     fv_tm (tapp_tm e2 (vfvar y)))
+    (res_product n my Hc).
 Proof.
   intros Hequiv Hdom Hrestrict Hworld.
-  pose proof (typed_total_tm_result_equiv_on_source_zero
-    Σ (CTArrow τx τr) m e1 e2 Hequiv) as Hzero1.
-  pose proof (typed_total_tm_result_equiv_on_target_zero
-    Σ (CTArrow τx τr) m e1 e2 Hequiv) as Hzero2.
-  pose proof (denot_ty_lvar_gas_guard_of_zero
-    Σ (CTArrow τx τr) e1 m Hzero1) as Hguard1.
-  pose proof (denot_ty_lvar_gas_guard_of_zero
-    Σ (CTArrow τx τr) e2 m Hzero2) as Hguard2.
+  pose proof (typed_total_equiv_source_zero
+    Σ (CTWand τx τr) m e1 e2 Hequiv) as Hzero1.
+  pose proof (typed_total_equiv_target_zero
+    Σ (CTWand τx τr) m e1 e2 Hequiv) as Hzero2.
+  pose proof (ty_denote_gas_guard_of_zero
+    Σ (CTWand τx τr) e1 m Hzero1) as Hguard1.
+  pose proof (ty_denote_gas_guard_of_zero
+    Σ (CTWand τx τr) e2 m Hzero2) as Hguard2.
   repeat rewrite res_models_and_iff in Hguard1.
   repeat rewrite res_models_and_iff in Hguard2.
   destruct Hguard1 as [_ [Hworld1 [Hbasic1 _]]].
@@ -178,8 +180,8 @@ Proof.
     rewrite <- Hrestrict.
     apply res_restrict_le.
   }
-  pose proof (typed_total_tm_result_equiv_on_term_scope
-    Σ (CTArrow τx τr) m e1 e2 Hequiv) as Hscope.
+  pose proof (typed_total_equiv_term_scope
+    Σ (CTWand τx τr) m e1 e2 Hequiv) as Hscope.
   assert (Hclosed1 : wfworld_closed_on (fv_tm e1) my).
   {
     eapply wfworld_closed_on_le.
@@ -209,26 +211,37 @@ Proof.
   }
   assert (Hclosed_y : wfworld_closed_on ({[y]} : aset) my).
   { eapply basic_world_formula_singleton_free_closed_on. exact Hworld_y. }
-  eapply (wfworld_closed_on_mono _
-    ((fv_tm e1 ∪ fv_tm e2) ∪ ({[y]} : aset)) my).
-  - rewrite !fv_tapp_tm. cbn [fv_value]. set_solver.
-  - apply (wfworld_closed_on_union (fv_tm e1 ∪ fv_tm e2) ({[y]} : aset)).
-    + apply (wfworld_closed_on_union (fv_tm e1) (fv_tm e2));
-        [exact Hclosed1|exact Hclosed2].
+  assert (Hclosed_my :
+      wfworld_closed_on
+        (fv_tm (tapp_tm e1 (vfvar y)) ∪
+         fv_tm (tapp_tm e2 (vfvar y))) my).
+  {
+    eapply (wfworld_closed_on_mono _
+      ((fv_tm e1 ∪ fv_tm e2) ∪ ({[y]} : aset)) my).
+    - rewrite !fv_tapp_tm. cbn [fv_value]. set_solver.
+    - apply (wfworld_closed_on_union (fv_tm e1 ∪ fv_tm e2) ({[y]} : aset)).
+      + apply (wfworld_closed_on_union (fv_tm e1) (fv_tm e2));
+          [exact Hclosed1|exact Hclosed2].
       + exact Hclosed_y.
+  }
+  eapply wfworld_closed_on_le.
+  - rewrite !fv_tapp_tm. cbn [fv_value].
+    rewrite Hdom. pose proof Hscope as Hscope'. set_solver.
+  - apply res_product_le_r.
+  - exact Hclosed_my.
 Qed.
 
-Lemma basic_world_formula_arrow_open_result_source_world
+Lemma basic_world_formula_wand_open_result_source_world
     (Σ : lty_env) τx τr e1 e2 (m my : WfWorldT) :
-  typed_total_tm_result_equiv_on Σ (CTArrow τx τr) m e1 e2 ->
+  typed_total_equiv_on Σ (CTWand τx τr) m e1 e2 ->
   res_restrict my (world_dom (m : WorldT)) = m ->
-  my ⊨ basic_world_formula (denot_relevant_env Σ (CTArrow τx τr) e2).
+  my ⊨ basic_world_formula (denot_relevant_env Σ (CTWand τx τr) e2).
 Proof.
   intros Hequiv Hrestrict.
-  pose proof (typed_total_tm_result_equiv_on_target_zero
-    Σ (CTArrow τx τr) m e1 e2 Hequiv) as Hzero_top_tgt.
-  pose proof (denot_ty_lvar_gas_guard_of_zero
-    Σ (CTArrow τx τr) e2 m Hzero_top_tgt) as Hguard_top_tgt.
+  pose proof (typed_total_equiv_target_zero
+    Σ (CTWand τx τr) m e1 e2 Hequiv) as Hzero_top_tgt.
+  pose proof (ty_denote_gas_guard_of_zero
+    Σ (CTWand τx τr) e2 m Hzero_top_tgt) as Hguard_top_tgt.
   repeat rewrite res_models_and_iff in Hguard_top_tgt.
   destruct Hguard_top_tgt as [_ [Hworld_top_tgt _]].
   assert (Hle : m ⊑ my).
@@ -236,63 +249,47 @@ Proof.
   eapply res_models_kripke; [exact Hle|exact Hworld_top_tgt].
 Qed.
 
-Lemma basic_world_formula_opened_arg_world
-    (Ty : ty) (my : WfWorldT) y :
-  my ⊨ formula_open 0 y
-    (basic_world_formula (<[LVBound 0 := Ty]> ∅)) ->
-  my ⊨ basic_world_formula
-    ((<[LVFree y := Ty]> (∅ : gmap logic_var ty)) : lty_env).
-Proof.
-  intros Hworld.
-  change (<[LVBound 0 := Ty]> (∅ : gmap logic_var ty))
-    with (typed_lty_env_bind (∅ : lty_env) Ty) in Hworld.
-  rewrite formula_open_basic_world_bind0 in Hworld.
-  - exact Hworld.
-  - set_solver.
-  - intros v Hv. set_solver.
-Qed.
-
-Lemma basic_world_formula_arrow_open_result_big
+Lemma basic_world_formula_wand_open_result_big
     (Σ : lty_env) τx τr e1 e2 (m my : WfWorldT) y :
-  typed_total_tm_result_equiv_on Σ (CTArrow τx τr) m e1 e2 ->
+  typed_total_equiv_on Σ (CTWand τx τr) m e1 e2 ->
   y ∉ fv_cty τx ->
   y ∉ fv_cty τr ->
   y ∉ fv_tm e1 ∪ fv_tm e2 ->
-  my ⊨ basic_world_formula (denot_relevant_env Σ (CTArrow τx τr) e2) ->
+  my ⊨ basic_world_formula (denot_relevant_env Σ (CTWand τx τr) e2) ->
   my ⊨ basic_world_formula
     ((<[LVFree y := erase_ty τx]> (∅ : gmap logic_var ty)) : lty_env) ->
   my ⊨ basic_world_formula
     (denot_relevant_env
       (<[LVFree y := erase_ty τx]>
-        (denot_relevant_env Σ (CTArrow τx τr) e2))
+        (denot_relevant_env Σ (CTWand τx τr) e2))
       (cty_open 0 y τr) (tapp_tm e2 (vfvar y))).
 Proof.
   intros Hequiv Hyτx Hyτr Hye Hworld_src Hworld_y.
   pose proof Hworld_src as Hworld_src_parts.
   apply basic_world_formula_models_iff in Hworld_src_parts as [Hlc_rel [_ _]].
-  pose proof (typed_total_tm_result_equiv_on_target_zero
-    Σ (CTArrow τx τr) m e1 e2 Hequiv) as Hzero_top_tgt.
-  pose proof (denot_ty_lvar_gas_guard_of_zero
-    Σ (CTArrow τx τr) e2 m Hzero_top_tgt) as Hguard_top_tgt.
+  pose proof (typed_total_equiv_target_zero
+    Σ (CTWand τx τr) m e1 e2 Hequiv) as Hzero_top_tgt.
+  pose proof (ty_denote_gas_guard_of_zero
+    Σ (CTWand τx τr) e2 m Hzero_top_tgt) as Hguard_top_tgt.
   repeat rewrite res_models_and_iff in Hguard_top_tgt.
   destruct Hguard_top_tgt as [Hwf_top_tgt _].
   apply context_ty_wf_formula_models_iff in Hwf_top_tgt
-    as [_ [_ Hbasic_arrow]].
-  eapply basic_world_formula_arrow_body_from_source_and_arg.
+    as [_ [_ Hbasic_wand]].
+  eapply basic_world_formula_wand_body_from_source_and_arg.
   - exact Hlc_rel.
-  - eapply denot_relevant_env_arrow_fresh_free.
+  - eapply denot_relevant_env_wand_fresh_free.
     + exact Hyτx.
     + exact Hyτr.
     + set_solver.
-  - exact Hbasic_arrow.
+  - exact Hbasic_wand.
   - apply tm_lvars_tapp_tm_fvar_without_arg.
   - rewrite denot_relevant_env_idemp. exact Hworld_src.
   - exact Hworld_y.
 Qed.
 
-Lemma basic_world_formula_arrow_open_result_subenv
+Lemma basic_world_formula_wand_open_result_subenv
     (Σ : lty_env) τx τr e1 e2 (m : WfWorldT) y :
-  typed_total_tm_result_equiv_on Σ (CTArrow τx τr) m e1 e2 ->
+  typed_total_equiv_on Σ (CTWand τx τr) m e1 e2 ->
   y ∉ fv_cty τx ->
   y ∉ fv_cty τr ->
   y ∉ fv_tm e1 ∪ fv_tm e2 ->
@@ -302,32 +299,29 @@ Lemma basic_world_formula_arrow_open_result_subenv
       (cty_open 0 y τr) (tapp_tm e2 (vfvar y)) !! v = Some T ->
     denot_relevant_env
       (<[LVFree y := erase_ty τx]>
-        (denot_relevant_env Σ (CTArrow τx τr) e2))
+        (denot_relevant_env Σ (CTWand τx τr) e2))
       (cty_open 0 y τr) (tapp_tm e2 (vfvar y)) !! v = Some T.
 Proof.
   intros Hequiv Hyτx Hyτr Hye v T Hlook.
-  pose proof (typed_total_tm_result_equiv_on_term_lc
-    Σ (CTArrow τx τr) m e1 e2 Hequiv) as [_ Hlc2].
-  pose proof (typed_total_tm_result_equiv_on_target_zero
-    Σ (CTArrow τx τr) m e1 e2 Hequiv) as Hzero_top_tgt.
-  pose proof (denot_ty_lvar_gas_guard_of_zero
-    Σ (CTArrow τx τr) e2 m Hzero_top_tgt) as Hguard_top_tgt.
+  pose proof (typed_total_equiv_term_lc
+    Σ (CTWand τx τr) m e1 e2 Hequiv) as [_ Hlc2].
+  pose proof (typed_total_equiv_target_zero
+    Σ (CTWand τx τr) m e1 e2 Hequiv) as Hzero_top_tgt.
+  pose proof (ty_denote_gas_guard_of_zero
+    Σ (CTWand τx τr) e2 m Hzero_top_tgt) as Hguard_top_tgt.
   repeat rewrite res_models_and_iff in Hguard_top_tgt.
   destruct Hguard_top_tgt as [Hwf_top_tgt _].
   apply context_ty_wf_formula_models_iff in Hwf_top_tgt
-    as [HlcΣ _].
-  assert (Hlc_rel :
-      lc_lvars (dom (denot_relevant_env Σ (CTArrow τx τr) e2 : lty_env))).
-  { exact HlcΣ. }
+    as [Hlc_rel _].
   assert (Hy_rel :
-      LVFree y ∉ dom (denot_relevant_env Σ (CTArrow τx τr) e2 : lty_env)).
+      LVFree y ∉ dom (denot_relevant_env Σ (CTWand τx τr) e2 : lty_env)).
   {
-    eapply denot_relevant_env_arrow_fresh_free.
+    eapply denot_relevant_env_wand_fresh_free.
     - exact Hyτx.
     - exact Hyτr.
     - set_solver.
   }
-  pose proof (arrow_body_relevant_env_agree_open_one_core
+  pose proof (wand_body_relevant_env_agree_open_one_core
     Σ (erase_ty τx) y τx τr e2 (tapp_tm e2 (vfvar y))
     Hyτr (tm_lvars_tapp_tm_fvar_without_arg_shift_lc e2 y Hlc2)) as Hagree.
   change ((lty_env_restrict_lvars
@@ -339,16 +333,16 @@ Proof.
     (exact Hy_rel || exact Hlc_rel).
   change ((lty_env_restrict_lvars
     (<[LVFree y := erase_ty τx]>
-      (denot_relevant_env Σ (CTArrow τx τr) e2))
+      (denot_relevant_env Σ (CTWand τx τr) e2))
     (denot_relevant_lvars (cty_open 0 y τr) (tapp_tm e2 (vfvar y)))
     : lty_env) !! v = Some T).
   exact Hlook.
 Qed.
 
-Lemma basic_world_formula_arrow_open_result_target
+Lemma basic_world_formula_wand_open_result_target
     gas (Σ : lty_env) τx τr e1 e2
-    (m my : WfWorldT) y :
-  typed_total_tm_result_equiv_on Σ (CTArrow τx τr) m e1 e2 ->
+    (m my n : WfWorldT) y (Hc : world_compat n my) :
+  typed_total_equiv_on Σ (CTWand τx τr) m e1 e2 ->
   world_dom (my : WorldT) = world_dom (m : WorldT) ∪ {[y]} ->
   res_restrict my (world_dom (m : WorldT)) = m ->
   y ∉ fv_cty τx ->
@@ -356,36 +350,44 @@ Lemma basic_world_formula_arrow_open_result_target
   y ∉ fv_tm e1 ∪ fv_tm e2 ->
   my ⊨ formula_open 0 y
     (basic_world_formula (<[LVBound 0 := erase_ty τx]> ∅)) ->
-  my ⊨ denot_ty_lvar_gas gas
+  res_product n my Hc ⊨ ty_denote_gas gas
     (lty_env_open_one 0 y (typed_lty_env_bind Σ (erase_ty τx)))
     (cty_open 0 y τr) (tapp_tm e1 (vfvar y)) ->
-  my ⊨ denot_ty_lvar_gas gas
+  n ⊨ ty_denote_gas gas
     (lty_env_open_one 0 y
       (typed_lty_env_bind
-        (denot_relevant_env Σ (CTArrow τx τr) e2)
+        (denot_relevant_env Σ (CTWand τx τr) e2)
         (erase_ty τx)))
     (cty_open 0 y (cty_shift 0 τx)) (tret (vfvar y)) ->
-  my ⊨ basic_world_formula
+  res_product n my Hc ⊨ basic_world_formula
     (denot_relevant_env
       (lty_env_open_one 0 y (typed_lty_env_bind Σ (erase_ty τx)))
       (cty_open 0 y τr) (tapp_tm e2 (vfvar y))).
 Proof.
   intros Hequiv Hdom Hrestrict Hyτx Hyτr Hye Hworld Hres_mid Harg.
-  pose proof (basic_world_formula_arrow_open_result_source_world
+  pose proof (basic_world_formula_wand_open_result_source_world
     Σ τx τr e1 e2 m my Hequiv Hrestrict) as Hworld_src_my.
+  assert (Hworld_src_prod :
+      res_product n my Hc ⊨
+        basic_world_formula (denot_relevant_env Σ (CTWand τx τr) e2)).
+  { eapply res_models_kripke; [apply res_product_le_r|exact Hworld_src_my]. }
   pose proof (basic_world_formula_opened_arg_world (erase_ty τx) my y Hworld)
-    as Hworld_y.
-  pose proof (basic_world_formula_arrow_open_result_big
-    Σ τx τr e1 e2 m my y Hequiv Hyτx Hyτr Hye
-    Hworld_src_my Hworld_y) as Hworld_big.
+    as Hworld_y_my.
+  assert (Hworld_y_prod :
+      res_product n my Hc ⊨ basic_world_formula
+        ((<[LVFree y := erase_ty τx]> (∅ : gmap logic_var ty)) : lty_env)).
+  { eapply res_models_kripke; [apply res_product_le_r|exact Hworld_y_my]. }
+  pose proof (basic_world_formula_wand_open_result_big
+    Σ τx τr e1 e2 m (res_product n my Hc) y
+    Hequiv Hyτx Hyτr Hye Hworld_src_prod Hworld_y_prod) as Hworld_big.
   eapply basic_world_formula_subenv; [|exact Hworld_big].
-  eapply basic_world_formula_arrow_open_result_subenv; eauto.
+  eapply basic_world_formula_wand_open_result_subenv; eauto.
 Qed.
 
-Lemma expr_basic_typing_formula_arrow_open_result_target
+Lemma expr_basic_typing_formula_wand_open_result_target
     gas (Σ : lty_env) τx τr e1 e2
-    (m my : WfWorldT) y :
-  typed_total_tm_result_equiv_on Σ (CTArrow τx τr) m e1 e2 ->
+    (m my n : WfWorldT) y (Hc : world_compat n my) :
+  typed_total_equiv_on Σ (CTWand τx τr) m e1 e2 ->
   world_dom (my : WorldT) = world_dom (m : WorldT) ∪ {[y]} ->
   res_restrict my (world_dom (m : WorldT)) = m ->
   y ∉ fv_cty τx ->
@@ -393,24 +395,24 @@ Lemma expr_basic_typing_formula_arrow_open_result_target
   y ∉ fv_tm e1 ∪ fv_tm e2 ->
   my ⊨ formula_open 0 y
     (basic_world_formula (<[LVBound 0 := erase_ty τx]> ∅)) ->
-  my ⊨ denot_ty_lvar_gas gas
+  res_product n my Hc ⊨ ty_denote_gas gas
     (lty_env_open_one 0 y (typed_lty_env_bind Σ (erase_ty τx)))
     (cty_open 0 y τr) (tapp_tm e1 (vfvar y)) ->
-  my ⊨ denot_ty_lvar_gas gas
+  n ⊨ ty_denote_gas gas
     (lty_env_open_one 0 y
       (typed_lty_env_bind
-        (denot_relevant_env Σ (CTArrow τx τr) e2)
+        (denot_relevant_env Σ (CTWand τx τr) e2)
         (erase_ty τx)))
     (cty_open 0 y (cty_shift 0 τx)) (tret (vfvar y)) ->
-  my ⊨ expr_basic_typing_formula
+  res_product n my Hc ⊨ expr_basic_typing_formula
     (denot_relevant_env
       (lty_env_open_one 0 y (typed_lty_env_bind Σ (erase_ty τx)))
       (cty_open 0 y τr) (tapp_tm e2 (vfvar y)))
     (tapp_tm e2 (vfvar y)) (erase_ty (cty_open 0 y τr)).
 Proof.
   intros Hequiv Hdom Hrestrict Hyτx Hyτr Hye Hworld Hres_mid Harg.
-  pose proof (basic_world_formula_arrow_open_result_target
-    gas Σ τx τr e1 e2 m my y Hequiv Hdom Hrestrict
+  pose proof (basic_world_formula_wand_open_result_target
+    gas Σ τx τr e1 e2 m my n y Hc Hequiv Hdom Hrestrict
     Hyτx Hyτr Hye Hworld Hres_mid Harg) as Hworld_tgt.
   apply expr_basic_typing_formula_models_iff.
   apply basic_world_formula_models_iff in Hworld_tgt
@@ -421,14 +423,14 @@ Proof.
   eapply basic_tm_has_ltype_tapp_tm_lvar.
   - exact Hlc_tgt.
   - eapply (basic_tm_has_ltype_open_result_target_fun
-      Σ (CTArrow τx τr) τx τr e1 e2 m y); eauto.
+      Σ (CTWand τx τr) τx τr e1 e2 m y); eauto.
   - apply basic_value_has_ltype_open_result_target_arg.
 Qed.
 
-Lemma denot_ty_lvar_gas_zero_arrow_open_result_target
+Lemma ty_denote_gas_zero_wand_open_result_target
     gas (Σ : lty_env) τx τr e1 e2
-    (m my : WfWorldT) y :
-  typed_total_tm_result_equiv_on Σ (CTArrow τx τr) m e1 e2 ->
+    (m my n : WfWorldT) y (Hc : world_compat n my) :
+  typed_total_equiv_on Σ (CTWand τx τr) m e1 e2 ->
   world_dom (my : WorldT) = world_dom (m : WorldT) ∪ {[y]} ->
   res_restrict my (world_dom (m : WorldT)) = m ->
   y ∉ fv_cty τx ->
@@ -436,35 +438,35 @@ Lemma denot_ty_lvar_gas_zero_arrow_open_result_target
   y ∉ fv_tm e1 ∪ fv_tm e2 ->
   my ⊨ formula_open 0 y
     (basic_world_formula (<[LVBound 0 := erase_ty τx]> ∅)) ->
-  my ⊨ denot_ty_lvar_gas gas
+  res_product n my Hc ⊨ ty_denote_gas gas
     (lty_env_open_one 0 y (typed_lty_env_bind Σ (erase_ty τx)))
     (cty_open 0 y τr) (tapp_tm e1 (vfvar y)) ->
-  my ⊨ denot_ty_lvar_gas gas
+  n ⊨ ty_denote_gas gas
     (lty_env_open_one 0 y
       (typed_lty_env_bind
-        (denot_relevant_env Σ (CTArrow τx τr) e2)
+        (denot_relevant_env Σ (CTWand τx τr) e2)
         (erase_ty τx)))
     (cty_open 0 y (cty_shift 0 τx)) (tret (vfvar y)) ->
-  my ⊨ denot_ty_lvar_gas 0
+  res_product n my Hc ⊨ ty_denote_gas 0
     (lty_env_open_one 0 y (typed_lty_env_bind Σ (erase_ty τx)))
     (cty_open 0 y τr) (tapp_tm e2 (vfvar y)).
 Proof.
   intros Hequiv Hdom Hrestrict Hyτx Hyτr Hye Hworld Hres_mid Harg.
-  pose proof (denot_ty_lvar_gas_guard gas
+  pose proof (ty_denote_gas_guard gas
     (lty_env_open_one 0 y (typed_lty_env_bind Σ (erase_ty τx)))
-    (cty_open 0 y τr) (tapp_tm e1 (vfvar y)) my Hres_mid)
-    as Hguard_res_src.
-  pose proof (denot_ty_lvar_gas_guard gas
+    (cty_open 0 y τr) (tapp_tm e1 (vfvar y))
+    (res_product n my Hc) Hres_mid) as Hguard_res_src.
+  pose proof (ty_denote_gas_guard gas
     (lty_env_open_one 0 y
       (typed_lty_env_bind
-        (denot_relevant_env Σ (CTArrow τx τr) e2)
+        (denot_relevant_env Σ (CTWand τx τr) e2)
         (erase_ty τx)))
-    (cty_open 0 y (cty_shift 0 τx)) (tret (vfvar y)) my Harg)
+    (cty_open 0 y (cty_shift 0 τx)) (tret (vfvar y)) n Harg)
     as Hguard_arg.
-  pose proof (typed_total_tm_result_equiv_on_target_zero
-    Σ (CTArrow τx τr) m e1 e2 Hequiv) as Hzero_top_tgt.
-  pose proof (denot_ty_lvar_gas_guard_of_zero
-    Σ (CTArrow τx τr) e2 m Hzero_top_tgt) as Hguard_top_tgt.
+  pose proof (typed_total_equiv_target_zero
+    Σ (CTWand τx τr) m e1 e2 Hequiv) as Hzero_top_tgt.
+  pose proof (ty_denote_gas_guard_of_zero
+    Σ (CTWand τx τr) e2 m Hzero_top_tgt) as Hguard_top_tgt.
   repeat rewrite res_models_and_iff in Hguard_res_src.
   repeat rewrite res_models_and_iff in Hguard_arg.
   repeat rewrite res_models_and_iff in Hguard_top_tgt.
@@ -476,54 +478,62 @@ Proof.
   assert (Hclosed_apps :
       wfworld_closed_on
         (fv_tm (tapp_tm e1 (vfvar y)) ∪
-         fv_tm (tapp_tm e2 (vfvar y))) my).
+         fv_tm (tapp_tm e2 (vfvar y)))
+        (res_product n my Hc)).
   {
-    eapply wfworld_closed_on_arrow_open_result_apps; eauto.
+    eapply wfworld_closed_on_wand_open_result_apps; eauto.
   }
   assert (Heq_apps :
-      tm_result_equiv_on my
+      tm_equiv_on (res_product n my Hc)
         (tapp_tm e1 (vfvar y)) (tapp_tm e2 (vfvar y))).
   {
-    pose proof (typed_total_tm_result_equiv_on_term_lc
-      Σ (CTArrow τx τr) m e1 e2 Hequiv) as [Hlc1 Hlc2].
-    eapply tm_result_equiv_on_tapp_fvar.
+    pose proof (typed_total_equiv_term_lc
+      Σ (CTWand τx τr) m e1 e2 Hequiv) as [Hlc1 Hlc2].
+    eapply tm_equiv_tapp_fvar.
     - exact Hclosed_apps.
     - exact Hlc1.
     - exact Hlc2.
-    - pose proof (typed_total_tm_result_equiv_on_term_scope
-        Σ (CTArrow τx τr) m e1 e2 Hequiv) as Hscope.
-      destruct Hequiv as [Heq_base _].
-      eapply tm_result_equiv_on_full_world_extend_fresh.
-      + exact Heq_base.
-      + exact Hscope.
-      + exact Hye.
-      + exact Hdom.
-      + exact Hrestrict.
+    - eapply tm_equiv_res_product_right.
+      + pose proof (typed_total_equiv_term_scope
+          Σ (CTWand τx τr) m e1 e2 Hequiv) as Hscope.
+        destruct Hequiv as [Heq_base _].
+        eapply tm_equiv_full_world_extend_fresh.
+        * exact Heq_base.
+        * exact Hscope.
+        * exact Hye.
+        * exact Hdom.
+        * exact Hrestrict.
+      + pose proof (typed_total_equiv_term_scope
+          Σ (CTWand τx τr) m e1 e2 Hequiv) as Hscope.
+        rewrite Hdom. set_solver.
   }
   assert (Htotal_tgt :
-      my ⊨ expr_total_formula (tapp_tm e2 (vfvar y))).
+      res_product n my Hc ⊨ expr_total_formula (tapp_tm e2 (vfvar y))).
   {
-    pose proof (typed_total_tm_result_equiv_on_term_lc
-      Σ (CTArrow τx τr) m e1 e2 Hequiv) as [_ Hlc2].
-    pose proof (typed_total_tm_result_equiv_on_term_scope
-      Σ (CTArrow τx τr) m e1 e2 Hequiv) as Hscope.
-    eapply tm_result_equiv_on_total.
+    pose proof (typed_total_equiv_term_lc
+      Σ (CTWand τx τr) m e1 e2 Hequiv) as [_ Hlc2].
+    pose proof (typed_total_equiv_term_scope
+      Σ (CTWand τx τr) m e1 e2 Hequiv) as Hscope.
+    eapply tm_equiv_total.
     - exact Heq_apps.
     - apply lc_tapp_tm; [exact Hlc2|constructor].
     - rewrite fv_tapp_tm. cbn [fv_value].
-      rewrite Hdom. set_solver.
+      pose proof (raw_le_dom (my : WorldT)
+        (res_product n my Hc : WorldT)
+        (res_product_le_r n my Hc)) as Hdom_le.
+      rewrite Hdom in Hdom_le. set_solver.
     - exact Htotal_res_src.
   }
   assert (Hworld_tgt :
-      my ⊨ basic_world_formula
+      res_product n my Hc ⊨ basic_world_formula
         (denot_relevant_env
           (lty_env_open_one 0 y (typed_lty_env_bind Σ (erase_ty τx)))
           (cty_open 0 y τr) (tapp_tm e2 (vfvar y)))).
   {
-    eapply basic_world_formula_arrow_open_result_target; eauto.
+    eapply basic_world_formula_wand_open_result_target; eauto.
   }
   assert (Hwf_tgt :
-      my ⊨ context_ty_wf_formula
+      res_product n my Hc ⊨ context_ty_wf_formula
         (denot_relevant_env
           (lty_env_open_one 0 y (typed_lty_env_bind Σ (erase_ty τx)))
           (cty_open 0 y τr) (tapp_tm e2 (vfvar y)))
@@ -542,15 +552,15 @@ Proof.
     store_normalize. set_solver.
   }
   assert (Hbasic_tgt :
-      my ⊨ expr_basic_typing_formula
+      res_product n my Hc ⊨ expr_basic_typing_formula
         (denot_relevant_env
           (lty_env_open_one 0 y (typed_lty_env_bind Σ (erase_ty τx)))
           (cty_open 0 y τr) (tapp_tm e2 (vfvar y)))
         (tapp_tm e2 (vfvar y)) (erase_ty (cty_open 0 y τr))).
   {
-    eapply expr_basic_typing_formula_arrow_open_result_target; eauto.
+    eapply expr_basic_typing_formula_wand_open_result_target; eauto.
   }
-  apply denot_ty_lvar_gas_zero_of_guard.
+  apply ty_denote_gas_zero_of_guard.
   repeat rewrite res_models_and_iff.
   split.
   - exact Hwf_tgt.
@@ -561,10 +571,10 @@ Proof.
       * exact Htotal_tgt.
 Qed.
 
-Lemma typed_total_tm_result_equiv_on_arrow_open_result_mid
+Lemma typed_total_equiv_wand_open_result_mid
     gas (Σ : lty_env) τx τr e1 e2
-    (m my : WfWorldT) y :
-  typed_total_tm_result_equiv_on Σ (CTArrow τx τr) m e1 e2 ->
+    (m my n : WfWorldT) y (Hc : world_compat n my) :
+  typed_total_equiv_on Σ (CTWand τx τr) m e1 e2 ->
   world_dom (my : WorldT) = world_dom (m : WorldT) ∪ {[y]} ->
   res_restrict my (world_dom (m : WorldT)) = m ->
   y ∉ fv_cty τx ->
@@ -572,51 +582,54 @@ Lemma typed_total_tm_result_equiv_on_arrow_open_result_mid
   y ∉ fv_tm e1 ∪ fv_tm e2 ->
   my ⊨ formula_open 0 y
     (basic_world_formula (<[LVBound 0 := erase_ty τx]> ∅)) ->
-  my ⊨ denot_ty_lvar_gas gas
+  res_product n my Hc ⊨ ty_denote_gas gas
     (lty_env_open_one 0 y (typed_lty_env_bind Σ (erase_ty τx)))
     (cty_open 0 y τr) (tapp_tm e1 (vfvar y)) ->
-  my ⊨ denot_ty_lvar_gas gas
+  n ⊨ ty_denote_gas gas
     (lty_env_open_one 0 y
       (typed_lty_env_bind
-        (denot_relevant_env Σ (CTArrow τx τr) e2)
+        (denot_relevant_env Σ (CTWand τx τr) e2)
         (erase_ty τx)))
     (cty_open 0 y (cty_shift 0 τx)) (tret (vfvar y)) ->
-  typed_total_tm_result_equiv_on
+  typed_total_equiv_on
     (lty_env_open_one 0 y (typed_lty_env_bind Σ (erase_ty τx)))
-    (cty_open 0 y τr) my
+    (cty_open 0 y τr) (res_product n my Hc)
     (tapp_tm e1 (vfvar y)) (tapp_tm e2 (vfvar y)).
 Proof.
   intros Hequiv Hdom Hrestrict Hyτx Hyτr Hye Hworld Hres_mid Harg.
-  pose proof (typed_total_tm_result_equiv_on_term_lc
-    Σ (CTArrow τx τr) m e1 e2 Hequiv) as [Hlc1 Hlc2].
+  pose proof (typed_total_equiv_term_lc
+    Σ (CTWand τx τr) m e1 e2 Hequiv) as [Hlc1 Hlc2].
   split.
-  - eapply tm_result_equiv_on_tapp_fvar.
-    + eapply (wfworld_closed_on_arrow_open_result_apps
-        Σ τx τr e1 e2 m my y); eauto.
+  - eapply tm_equiv_tapp_fvar.
+    + eapply (wfworld_closed_on_wand_open_result_apps
+        Σ τx τr e1 e2 m my n y Hc); eauto.
     + exact Hlc1.
     + exact Hlc2.
-    + eapply tm_result_equiv_on_full_world_extend_fresh.
-      * exact (proj1 Hequiv).
-      * eapply typed_total_tm_result_equiv_on_term_scope. exact Hequiv.
-      * exact Hye.
-      * exact Hdom.
-      * exact Hrestrict.
+    + eapply tm_equiv_res_product_right.
+      * eapply tm_equiv_full_world_extend_fresh.
+        -- exact (proj1 Hequiv).
+        -- eapply typed_total_equiv_term_scope. exact Hequiv.
+        -- exact Hye.
+        -- exact Hdom.
+        -- exact Hrestrict.
+      * pose proof (typed_total_equiv_term_scope
+          Σ (CTWand τx τr) m e1 e2 Hequiv) as Hscope.
+        set_solver.
   - split.
-    + apply denot_ty_lvar_gas_zero_of_guard.
-      eapply denot_ty_lvar_gas_guard. exact Hres_mid.
-    + eapply (denot_ty_lvar_gas_zero_arrow_open_result_target
-        gas Σ τx τr e1 e2 m my y); eauto.
-  all: eauto.
+    + apply ty_denote_gas_zero_of_guard.
+      eapply ty_denote_gas_guard. exact Hres_mid.
+    + eapply (ty_denote_gas_zero_wand_open_result_target
+        gas Σ τx τr e1 e2 m my n y Hc); eauto.
 Qed.
 
-Lemma denot_ty_lvar_gas_tm_result_equiv_arrow_open_result
+Lemma ty_denote_gas_tm_equiv_wand_open_result
     gas (IH : forall Σ τ e1 e2 (m : WfWorldT),
-      typed_total_tm_result_equiv_on Σ τ m e1 e2 ->
-      m ⊨ denot_ty_lvar_gas gas Σ τ e1 ->
-      m ⊨ denot_ty_lvar_gas gas Σ τ e2)
+      typed_total_equiv_on Σ τ m e1 e2 ->
+      m ⊨ ty_denote_gas gas Σ τ e1 ->
+      m ⊨ ty_denote_gas gas Σ τ e2)
     (Σ : lty_env) τx τr e1 e2
-    (m my : WfWorldT) y :
-  typed_total_tm_result_equiv_on Σ (CTArrow τx τr) m e1 e2 ->
+    (m my n : WfWorldT) y (Hc : world_compat n my) :
+  typed_total_equiv_on Σ (CTWand τx τr) m e1 e2 ->
   world_dom (my : WorldT) = world_dom (m : WorldT) ∪ {[y]} ->
   res_restrict my (world_dom (m : WorldT)) = m ->
   y ∉ fv_cty τx ->
@@ -624,34 +637,34 @@ Lemma denot_ty_lvar_gas_tm_result_equiv_arrow_open_result
   y ∉ fv_tm e1 ∪ fv_tm e2 ->
   y ∉ lvars_fv
     (dom (typed_lty_env_bind
-      (denot_relevant_env Σ (CTArrow τx τr) e1) (erase_ty τx))) ->
+      (denot_relevant_env Σ (CTWand τx τr) e1) (erase_ty τx))) ->
   y ∉ lvars_fv
     (dom (typed_lty_env_bind
-      (denot_relevant_env Σ (CTArrow τx τr) e2) (erase_ty τx))) ->
+      (denot_relevant_env Σ (CTWand τx τr) e2) (erase_ty τx))) ->
   my ⊨ formula_open 0 y
     (basic_world_formula (<[LVBound 0 := erase_ty τx]> ∅)) ->
-  my ⊨ formula_open 0 y
-    (denot_ty_lvar_gas gas
+  n ⊨ formula_open 0 y
+    (ty_denote_gas gas
       (typed_lty_env_bind
-        (denot_relevant_env Σ (CTArrow τx τr) e2)
+        (denot_relevant_env Σ (CTWand τx τr) e2)
         (erase_ty τx))
       (cty_shift 0 τx) (tret (vbvar 0))) ->
-  my ⊨ formula_open 0 y
-    (denot_ty_lvar_gas gas
+  res_product n my Hc ⊨ formula_open 0 y
+    (ty_denote_gas gas
       (typed_lty_env_bind
-        (denot_relevant_env Σ (CTArrow τx τr) e1)
+        (denot_relevant_env Σ (CTWand τx τr) e1)
         (erase_ty τx))
       τr (tapp_tm (tm_shift 0 e1) (vbvar 0))) ->
-  my ⊨ formula_open 0 y
-    (denot_ty_lvar_gas gas
+  res_product n my Hc ⊨ formula_open 0 y
+    (ty_denote_gas gas
       (typed_lty_env_bind
-        (denot_relevant_env Σ (CTArrow τx τr) e2)
+        (denot_relevant_env Σ (CTWand τx τr) e2)
         (erase_ty τx))
       τr (tapp_tm (tm_shift 0 e2) (vbvar 0))).
 Proof.
   intros Hequiv Hdom Hrestrict Hyτx Hyτr Hye HyΣ1 HyΣ2 Hworld Harg Hres.
-  pose proof (typed_total_tm_result_equiv_on_term_lc
-    Σ (CTArrow τx τr) m e1 e2 Hequiv) as [Hlc1 Hlc2].
+  pose proof (typed_total_equiv_term_lc
+    Σ (CTWand τx τr) m e1 e2 Hequiv) as [Hlc1 Hlc2].
   assert (Hτa_fresh : y ∉ fv_cty (cty_shift 0 τx)).
   { rewrite cty_shift_fv. exact Hyτx. }
   assert (Harg_tm_fresh : y ∉ fv_tm (tret (vbvar 0))).
@@ -668,21 +681,21 @@ Proof.
     rewrite fv_tapp_tm, tm_shift_fv.
     cbn [fv_value]. set_solver.
   }
-  rewrite (formula_open_denot_ty_lvar_gas_singleton 0 y gas
+  rewrite (formula_open_ty_denote_gas_singleton 0 y gas
     (typed_lty_env_bind
-      (denot_relevant_env Σ (CTArrow τx τr) e1) (erase_ty τx))
+      (denot_relevant_env Σ (CTWand τx τr) e1) (erase_ty τx))
     τr (tapp_tm (tm_shift 0 e1) (vbvar 0))) in Hres
     by (exact HyΣ1 || exact Hsrc_tm_fresh || exact Hyτr).
-  rewrite (formula_open_denot_ty_lvar_gas_singleton 0 y gas
+  rewrite (formula_open_ty_denote_gas_singleton 0 y gas
     (typed_lty_env_bind
-      (denot_relevant_env Σ (CTArrow τx τr) e2) (erase_ty τx))
+      (denot_relevant_env Σ (CTWand τx τr) e2) (erase_ty τx))
     τr (tapp_tm (tm_shift 0 e2) (vbvar 0)))
     by (exact HyΣ2 || exact Htgt_tm_fresh || exact Hyτr).
   rewrite open_tapp_tm_shift_bvar0_lc in Hres by exact Hlc1.
   rewrite open_tapp_tm_shift_bvar0_lc by exact Hlc2.
-  rewrite (formula_open_denot_ty_lvar_gas_singleton 0 y gas
+  rewrite (formula_open_ty_denote_gas_singleton 0 y gas
     (typed_lty_env_bind
-      (denot_relevant_env Σ (CTArrow τx τr) e2) (erase_ty τx))
+      (denot_relevant_env Σ (CTWand τx τr) e2) (erase_ty τx))
     (cty_shift 0 τx) (tret (vbvar 0))) in Harg
     by (exact HyΣ2 || exact Harg_tm_fresh || exact Hτa_fresh).
   replace (open_tm 0 (vfvar y) (tret (vbvar 0))) with
@@ -693,107 +706,106 @@ Proof.
   set (etgt := tapp_tm e2 (vfvar y)).
   fold τres esrc etgt in Hres |- *.
   assert (Hres_mid :
-      my ⊨ denot_ty_lvar_gas gas
+      res_product n my Hc ⊨ ty_denote_gas gas
         (lty_env_open_one 0 y (typed_lty_env_bind Σ (erase_ty τx)))
         τres esrc).
   {
     unfold τres, esrc.
-    eapply denot_ty_lvar_gas_tm_result_equiv_arrow_open_result_source_mid;
+    eapply ty_denote_gas_tm_equiv_wand_open_result_source_mid;
       eauto.
   }
   assert (Htgt_mid_to_goal :
-      my ⊨ denot_ty_lvar_gas gas
+      res_product n my Hc ⊨ ty_denote_gas gas
         (lty_env_open_one 0 y (typed_lty_env_bind Σ (erase_ty τx)))
         τres etgt ->
-      my ⊨ denot_ty_lvar_gas gas
+      res_product n my Hc ⊨ ty_denote_gas gas
         (lty_env_open_one 0 y
           (typed_lty_env_bind
-            (denot_relevant_env Σ (CTArrow τx τr) e2)
+            (denot_relevant_env Σ (CTWand τx τr) e2)
             (erase_ty τx)))
         τres etgt).
   {
     unfold τres, etgt.
-    eapply denot_ty_lvar_gas_tm_result_equiv_arrow_open_result_target_mid_to_goal;
+    eapply ty_denote_gas_tm_equiv_wand_open_result_target_mid_to_goal;
       eauto.
   }
   apply Htgt_mid_to_goal.
   eapply IH.
   - unfold τres, esrc, etgt in *.
-    eapply typed_total_tm_result_equiv_on_arrow_open_result_mid; eauto.
+    eapply typed_total_equiv_wand_open_result_mid; eauto.
   - exact Hres_mid.
 Qed.
 
-
-Lemma denot_ty_lvar_gas_tm_result_equiv_arrow_body
+Lemma ty_denote_gas_tm_equiv_wand_body
     gas (IH : forall Σ τ e1 e2 (m : WfWorldT),
-      typed_total_tm_result_equiv_on Σ τ m e1 e2 ->
-      m ⊨ denot_ty_lvar_gas gas Σ τ e1 ->
-      m ⊨ denot_ty_lvar_gas gas Σ τ e2)
+      typed_total_equiv_on Σ τ m e1 e2 ->
+      m ⊨ ty_denote_gas gas Σ τ e1 ->
+      m ⊨ ty_denote_gas gas Σ τ e2)
     (Σ : lty_env) τx τr e1 e2 (m : WfWorldT) :
-  typed_total_tm_result_equiv_on Σ (CTArrow τx τr) m e1 e2 ->
+  typed_total_equiv_on Σ (CTWand τx τr) m e1 e2 ->
   m ⊨
     FForall
       (FImpl (basic_world_formula (<[LVBound 0 := erase_ty τx]> ∅))
-        (FImpl
-          (denot_ty_lvar_gas gas
+        (FWand
+          (ty_denote_gas gas
             (typed_lty_env_bind
-              (denot_relevant_env Σ (CTArrow τx τr) e1)
+              (denot_relevant_env Σ (CTWand τx τr) e1)
               (erase_ty τx))
             (cty_shift 0 τx) (tret (vbvar 0)))
-          (denot_ty_lvar_gas gas
+          (ty_denote_gas gas
             (typed_lty_env_bind
-              (denot_relevant_env Σ (CTArrow τx τr) e1)
+              (denot_relevant_env Σ (CTWand τx τr) e1)
               (erase_ty τx))
             τr (tapp_tm (tm_shift 0 e1) (vbvar 0))))) ->
   m ⊨
     FForall
       (FImpl (basic_world_formula (<[LVBound 0 := erase_ty τx]> ∅))
-        (FImpl
-          (denot_ty_lvar_gas gas
+        (FWand
+          (ty_denote_gas gas
             (typed_lty_env_bind
-              (denot_relevant_env Σ (CTArrow τx τr) e2)
+              (denot_relevant_env Σ (CTWand τx τr) e2)
               (erase_ty τx))
             (cty_shift 0 τx) (tret (vbvar 0)))
-          (denot_ty_lvar_gas gas
+          (ty_denote_gas gas
             (typed_lty_env_bind
-              (denot_relevant_env Σ (CTArrow τx τr) e2)
+              (denot_relevant_env Σ (CTWand τx τr) e2)
               (erase_ty τx))
             τr (tapp_tm (tm_shift 0 e2) (vbvar 0))))).
 Proof.
   intros Hequiv Hsrc.
-  pose proof (typed_total_tm_result_equiv_on_target_zero
-    Σ (CTArrow τx τr) m e1 e2 Hequiv) as Hzero_tgt.
-  pose proof (denot_ty_lvar_gas_guard_of_zero
-    Σ (CTArrow τx τr) e2 m Hzero_tgt) as Hguard_tgt.
+  pose proof (typed_total_equiv_target_zero
+    Σ (CTWand τx τr) m e1 e2 Hequiv) as Hzero_tgt.
+  pose proof (ty_denote_gas_guard_of_zero
+    Σ (CTWand τx τr) e2 m Hzero_tgt) as Hguard_tgt.
   assert (Hscope_tgt :
       formula_scoped_in_world m
-        (denot_ty_lvar_gas (S gas) Σ (CTArrow τx τr) e2)).
+        (ty_denote_gas (S gas) Σ (CTWand τx τr) e2)).
   {
     unfold formula_scoped_in_world.
-    eapply formula_fv_denot_ty_lvar_gas_scope_from_guard_pre_open;
+    eapply formula_fv_ty_denote_gas_scope_from_guard_pre_open;
       [reflexivity|exact Hguard_tgt].
   }
-  cbn [denot_ty_lvar_gas] in Hscope_tgt.
+  cbn [ty_denote_gas] in Hscope_tgt.
   pose proof (formula_scoped_and_r _ _ _ Hscope_tgt) as Hbody_scope.
-  eapply res_models_forall_full_world_impl2_map_dep;
+  eapply res_models_forall_full_world_impl_wand_map_dep;
     [exact Hbody_scope| |exact Hsrc].
   exists (fv_cty τx ∪
     fv_cty τr ∪ fv_tm e1 ∪ fv_tm e2 ∪
     lvars_fv
       (dom (typed_lty_env_bind
-        (denot_relevant_env Σ (CTArrow τx τr) e1) (erase_ty τx))) ∪
+        (denot_relevant_env Σ (CTWand τx τr) e1) (erase_ty τx))) ∪
     lvars_fv
       (dom (typed_lty_env_bind
-        (denot_relevant_env Σ (CTArrow τx τr) e2) (erase_ty τx)))).
+        (denot_relevant_env Σ (CTWand τx τr) e2) (erase_ty τx)))).
   intros y Hy my Hdom Hrestrict.
   split; [intros Hworld; exact Hworld|].
   split.
-  - intros Harg.
-    eapply denot_ty_lvar_gas_tm_result_equiv_arrow_open_arg; eauto;
+  - intros n Hc Harg.
+    eapply ty_denote_gas_tm_equiv_wand_open_arg; eauto;
       set_solver.
-  - intros Hworld Harg Hres.
-    eapply denot_ty_lvar_gas_tm_result_equiv_arrow_open_result; eauto.
+  - intros Hworld n Hc Harg Hres.
+    eapply ty_denote_gas_tm_equiv_wand_open_result; eauto.
     all: set_solver.
 Qed.
 
-End ContextTypeDenotation.
+End TypeDenote.
